safe point

NuSys.thy
@@ -154,7 +154,7 @@ qed
 
 
 
-section \<open>Mechanisms - I\<close>
+section \<open>Mechanisms - I - Preludes\<close>
 
 subsection \<open>Congruence Rule\<close>
 
@@ -198,6 +198,9 @@ lemma cast_id[\<nu>intro 2000]: "\<^bold>c\<^bold>a\<^bold>s\<^bold>t A \<longma
 lemma cast_dual_id[\<nu>intro 2000]: "\<^bold>c\<^bold>a\<^bold>s\<^bold>t A \<longmapsto> A \<^bold>d\<^bold>u\<^bold>a\<^bold>l B \<longmapsto> B"
   unfolding CastDual_def Intro_def Dest_def by (simp add: cast_id)
 
+lemma CastDual_I:
+  "\<^bold>c\<^bold>a\<^bold>s\<^bold>t A \<longmapsto> B \<^bold>w\<^bold>i\<^bold>t\<^bold>h P \<Longrightarrow> \<^bold>c\<^bold>a\<^bold>s\<^bold>t B' \<longmapsto> A' \<^bold>w\<^bold>i\<^bold>t\<^bold>h Any \<Longrightarrow> \<^bold>c\<^bold>a\<^bold>s\<^bold>t A \<longmapsto> B \<^bold>w\<^bold>i\<^bold>t\<^bold>h P \<^bold>d\<^bold>u\<^bold>a\<^bold>l B' \<longmapsto> A' "
+  unfolding CastDual_def Cast_def by blast
 
 text \<open>There are 3 kinds of the Cast, corresponding 3 usages where the prefix `some_`
 means the variable *can* be schematic (which is unknown in the reasoning) while other variables
@@ -346,15 +349,12 @@ end
 
 subsubsection \<open>Abstractor\<close>
 
-definition NuVoid :: "(void, unit) \<nu>" where "NuVoid _ = UNIV"
+definition Void :: " void set " where "Void = UNIV"
 text \<open>The name `void` coincides that, when a procedure has no input arguments,
   the \<nu>-type for the input would exactly be @{term Void}. \<close>
 
-consts Void_sugar :: " 'a_sugar " ("Void")
-translations "Void" == "() \<tycolon> CONST NuVoid"
-
-lemma [nu_exps]: "p \<nuLinkL> NuVoid \<nuLinkR> x" unfolding NuVoid_def Refining_def by simp
-lemma [elim!, \<nu>elim]: "Inhabited \<tort_lbrace>Void\<tort_rbrace> \<Longrightarrow> C \<Longrightarrow> C" by simp
+lemma [nu_exps]: "p \<in> Void" unfolding Void_def by simp
+lemma [elim!, \<nu>elim]: "Inhabited Void \<Longrightarrow> C \<Longrightarrow> C" by simp
 (*translations "a" <= "a \<^bold>a\<^bold>n\<^bold>d CONST Void"*)
 
 subsection \<open>Prod & the pair abstract structure\<close>
@@ -392,16 +392,16 @@ lemma Separation_exp[nu_exps]: "h \<nuLinkL> A \<^emph> B \<nuLinkR> (a,b) \<lon
   (\<exists>h2 h1. h = h2 ++ h1 \<and> dom h2 \<perpendicular> dom h1 \<and> (h1 \<nuLinkL> A \<nuLinkR> a) \<and> (h2 \<nuLinkL> B \<nuLinkR> b))"
   unfolding Separation_def Refining_def by simp
 
-definition Heap_Delimiter :: "(heap,'ax) \<nu> \<Rightarrow> (heap,'bx) \<nu> \<Rightarrow> (heap, 'ax \<times> 'bx) \<nu>" (infixr "<heap-sep>" 70)
-  where "A <heap-sep> B = A \<^emph> B"
-consts Heap_Delimiter_sugar :: " 'just \<Rightarrow> 'a \<Rightarrow> 'sugar " ( "_/ \<heavy_asterisk> _" [14,15] 14) \<comment> \<open>It is left associative!\<close>
+definition Heap_Divider :: "heap set \<Rightarrow> heap set \<Rightarrow> heap set" ( "_/ \<heavy_asterisk> _" [14,15] 14)
+  where "(A \<heavy_asterisk> B) = {h. (\<exists>h1 h2. h = h1 ++ h2 \<and> dom h1 \<perpendicular> dom h2 \<and> (h1 \<in> A) \<and> (h2 \<in> B))}"
+translations " A \<heavy_asterisk> (b \<tycolon> B) " \<rightleftharpoons> " A \<heavy_asterisk> \<tort_lbrace> b \<tycolon> B \<tort_rbrace> "
+  " (a \<tycolon> A) \<heavy_asterisk> B " \<rightleftharpoons> " \<tort_lbrace>a \<tycolon> A\<tort_rbrace> \<heavy_asterisk> B "
 
-translations " (a \<tycolon> A) \<heavy_asterisk> (b \<tycolon> B) " \<rightleftharpoons> " (CONST Pair b a) \<tycolon> (B <heap-sep> A) "
-  " A \<heavy_asterisk> B " => " (CONST Pair (_\<nu>typing_x B) (_\<nu>typing_x A)) \<tycolon> ((_\<nu>typing_ty B) <heap-sep> (_\<nu>typing_ty A)) "
-
-lemma Heap_Delimiter_cong: "\<tort_lbrace>h1 \<tycolon> H1\<tort_rbrace> \<equiv> \<tort_lbrace>h1' \<tycolon> H1'\<tort_rbrace> \<Longrightarrow> \<tort_lbrace>h2 \<tycolon> H2\<tort_rbrace> \<equiv> \<tort_lbrace>h2' \<tycolon> H2'\<tort_rbrace> \<Longrightarrow> \<tort_lbrace>h1 \<tycolon> H1 \<heavy_asterisk> h2 \<tycolon> H2\<tort_rbrace> \<equiv> \<tort_lbrace>h1' \<tycolon> H1' \<heavy_asterisk> h2' \<tycolon> H2'\<tort_rbrace>"
-  unfolding atomize_eq Heap_Delimiter_def by (auto 0 5 simp add: nu_exps)
-simproc_setup Heap_Delimiter_cong ("\<tort_lbrace>h1 \<tycolon> H1 \<heavy_asterisk> h2 \<tycolon> H2\<tort_rbrace>") = \<open>K (NuSimpCong.simproc @{thm Heap_Delimiter_cong})\<close>
+lemma Heap_Divider_exps[nu_exps]:
+  "h \<in> (A \<heavy_asterisk> B) \<longleftrightarrow> (\<exists>h1 h2. h = h1 ++ h2 \<and> dom h1 \<perpendicular> dom h2 \<and> (h1 \<in> A) \<and> (h2 \<in> B))"
+  unfolding Heap_Divider_def by simp
+lemma SepNu_to_SepSet: "\<tort_lbrace>(a,b) \<tycolon> A \<^emph> B\<tort_rbrace> = (b \<tycolon> B \<heavy_asterisk> a \<tycolon> A)"
+  unfolding Heap_Divider_def by (auto 0 3 simp add: Separation_exp)
 
 
 
@@ -431,24 +431,13 @@ lemma heap_split_by_addr_set: "P (h |` (MemAddress ` S)) (h |` (- (MemAddress ` 
 
 
 
+lemma Separation_comm: " (A \<heavy_asterisk> B) = (B \<heavy_asterisk> A)" unfolding Heap_Divider_def
+  by (auto simp add: disjoint_def inf_commute dest: map_add_comm )
 
-definition SeparationSet :: " heap set \<Rightarrow> heap set \<Rightarrow> heap set" (infixr "<sep-set>" 70)
-  where "A <sep-set> B = {h. (\<exists>h1 h2. h = h1 ++ h2 \<and> dom h1 \<perpendicular> dom h2 \<and> h1 \<in> A \<and> h2 \<in> B)}"
-lemma HeapDivNu_to_SepSet: "\<tort_lbrace> h1 \<tycolon> H1 \<heavy_asterisk> h2 \<tycolon> H2 \<tort_rbrace> = \<tort_lbrace> h1 \<tycolon> H1 \<tort_rbrace> <sep-set> \<tort_lbrace> h2 \<tycolon> H2 \<tort_rbrace>"
-  unfolding SeparationSet_def Heap_Delimiter_def by (auto 4 4 simp add: nu_exps)
-lemma SepNu_to_SepSet: "\<tort_lbrace> (h2,h1) \<tycolon> H2 \<^emph> H1 \<tort_rbrace> = \<tort_lbrace> h1 \<tycolon> H1 \<tort_rbrace> <sep-set> \<tort_lbrace> h2 \<tycolon> H2 \<tort_rbrace>"
-  unfolding SeparationSet_def Heap_Delimiter_def by (auto 4 4 simp add: nu_exps)
-
-lemma SeparationSet_comm: " A <sep-set> B = B <sep-set> A" unfolding SeparationSet_def
-  by (auto 4 4 simp add: disjoint_def inf_commute dest: map_add_comm )
-lemma Separation_comm: " \<tort_lbrace> A \<heavy_asterisk> B\<tort_rbrace> = \<tort_lbrace> B \<heavy_asterisk> A\<tort_rbrace>"
-  unfolding HeapDivNu_to_SepSet using SeparationSet_comm by fast
-
-lemma SeparationSet_assoc: " (A <sep-set> B) <sep-set> C = A <sep-set> B <sep-set> C"
-  unfolding SeparationSet_def
-  by (auto simp add: disjoint_def) (metis (no_types, lifting) Un_empty dom_map_add inf_sup_distrib1 inf_sup_distrib2 map_add_assoc)+
-lemma Separation_assoc: "\<tort_lbrace> A \<heavy_asterisk> (B \<heavy_asterisk> C)\<tort_rbrace> = \<tort_lbrace> A \<heavy_asterisk> B \<heavy_asterisk> C\<tort_rbrace>"
-  unfolding HeapDivNu_to_SepSet using SeparationSet_assoc by fast
+lemma Separation_assoc: " (A \<heavy_asterisk> (B \<heavy_asterisk> C)) = (A \<heavy_asterisk> B \<heavy_asterisk> C)"
+  unfolding Heap_Divider_def apply (auto simp add: disjoint_def)
+  apply blast
+  by (smt (verit, del_insts) dom_map_add inf_commute inf_sup_absorb inf_sup_distrib1 map_add_assoc sup_bot_left)
 
 (* lemma NonSeparation_distrib_L: "h \<in> (A \<heavy_asterisk> (B \<dbl_and> P)) \<Longrightarrow> h \<in> (A \<heavy_asterisk> B \<dbl_and> P)"
   using map_le_map_add map_le_trans by blast
@@ -456,31 +445,27 @@ lemma NonSeparation_distrib_R: "h \<in> ((A \<dbl_and> P) \<heavy_asterisk> B) \
   by (metis NonSeparation_distrib_L Separation_comm) *)
   
 
-lemma [elim!,\<nu>elim]: "Inhabited \<tort_lbrace>a \<tycolon> A \<heavy_asterisk> b \<tycolon> B\<tort_rbrace> \<Longrightarrow> (a \<ratio> A \<Longrightarrow> b \<ratio> B \<Longrightarrow> C) \<Longrightarrow> C"
-  unfolding Inhabited_def Heap_Delimiter_def by (simp add: nu_exps) blast
+lemma [elim!,\<nu>elim]: "Inhabited (A \<heavy_asterisk> B) \<Longrightarrow> (Inhabited A \<Longrightarrow> Inhabited B \<Longrightarrow> C) \<Longrightarrow> C"
+  unfolding Inhabited_def Heap_Divider_def by (simp add: nu_exps) blast
 (* lemma [elim!,\<nu>elim]: "Inhabited (A \<dbl_and> B) \<Longrightarrow> (Inhabited A \<Longrightarrow> Inhabited B \<Longrightarrow> C) \<Longrightarrow> C"
   unfolding Inhabited_def by auto *)
 
 subsection \<open>Top Context\<close> \<comment> \<open>The pair of heap and stack\<close>
 
-definition NuTopCtx :: " (heap, 'hx) \<nu> \<Rightarrow> ('s :: stack, 'sx) \<nu> \<Rightarrow> (heap \<times> 's, 'hx \<times> 'sx) \<nu> " (infix "<top-ctx>" 59)
-  where "(H <top-ctx> S) = (\<lambda>(h,s). {(hp,sp). (hp \<nuLinkL> H \<nuLinkR> h) \<and> (sp \<nuLinkL> S \<nuLinkR> s) \<and> Heap hp})"
-consts "NuTopCtx_sugar" :: " 'just \<Rightarrow> 'a \<Rightarrow> 'sugar " ( "_ \<heavy_comma>/ \<^bold>h\<^bold>e\<^bold>a\<^bold>p _" [10,14] 13)
-translations "(s \<tycolon> S\<heavy_comma> \<^bold>h\<^bold>e\<^bold>a\<^bold>p h \<tycolon> H)" \<rightleftharpoons> "(CONST Pair h s) \<tycolon> CONST NuTopCtx H S"
-  "(S\<heavy_comma> \<^bold>h\<^bold>e\<^bold>a\<^bold>p H)" => "(_\<nu>typing_x H, _\<nu>typing_x S) \<tycolon> CONST NuTopCtx (_\<nu>typing_ty H) (_\<nu>typing_ty S)"
+definition NuTopCtx :: " 's :: stack set \<Rightarrow> heap set \<Rightarrow> (heap \<times> 's) set " (infix "<top-ctx>" 59)
+  where "(S <top-ctx> H) = {(h,s). Heap h \<and> h \<in> H \<and> s \<in> S}"
+notation NuTopCtx ( "_ \<heavy_comma>/ \<^bold>h\<^bold>e\<^bold>a\<^bold>p _" [10,14] 13)
 
-lemma [nu_exps]: " ((hp, sp) \<nuLinkL> H <top-ctx> S  \<nuLinkR> (h, s)) \<longleftrightarrow> (hp \<nuLinkL> H  \<nuLinkR> h) \<and> (sp \<nuLinkL> S  \<nuLinkR> s) \<and> Heap hp"
-  unfolding NuTopCtx_def Refining_def by simp
-lemma [elim!,\<nu>elim]: "Inhabited \<tort_lbrace>s \<tycolon> S \<heavy_comma> \<^bold>h\<^bold>e\<^bold>a\<^bold>p h \<tycolon> H\<tort_rbrace> \<Longrightarrow> (s \<ratio> S \<Longrightarrow> h \<ratio> H \<Longrightarrow> C) \<Longrightarrow> C"
+translations "(s \<tycolon> S) <top-ctx> H" \<rightleftharpoons> "\<tort_lbrace>s \<tycolon> S\<tort_rbrace> <top-ctx> H"
+  "S <top-ctx> (h \<tycolon> H)" \<rightleftharpoons> "S <top-ctx> \<tort_lbrace>h \<tycolon> H\<tort_rbrace>"
+
+lemma [nu_exps]: "(h,s) \<in> (S <top-ctx> H) \<longleftrightarrow> Heap h \<and> h \<in> H \<and> s \<in> S"
+  unfolding NuTopCtx_def by simp
+lemma [elim!,\<nu>elim]: "Inhabited (S \<heavy_comma> \<^bold>h\<^bold>e\<^bold>a\<^bold>p H) \<Longrightarrow> (Inhabited S \<Longrightarrow> Inhabited H \<Longrightarrow> C) \<Longrightarrow> C"
   unfolding Inhabited_def by (simp add: nu_exps) blast
 
-lemma NuTopCtx_cong: "\<tort_lbrace>h \<tycolon> H\<tort_rbrace> \<equiv> \<tort_lbrace>h' \<tycolon> H'\<tort_rbrace> \<Longrightarrow> \<tort_lbrace>s \<tycolon> S\<tort_rbrace> \<equiv> \<tort_lbrace>s' \<tycolon> S'\<tort_rbrace> \<Longrightarrow> \<tort_lbrace>s \<tycolon> S\<heavy_comma> \<^bold>h\<^bold>e\<^bold>a\<^bold>p h \<tycolon> H\<tort_rbrace> \<equiv> \<tort_lbrace>s' \<tycolon> S'\<heavy_comma> \<^bold>h\<^bold>e\<^bold>a\<^bold>p h' \<tycolon> H'\<tort_rbrace>"
-  unfolding atomize_eq by (auto 0 3 simp add: nu_exps)
-simproc_setup NuTopCtx_cong ("\<tort_lbrace>s \<tycolon> S \<heavy_comma> \<^bold>h\<^bold>e\<^bold>a\<^bold>p h \<tycolon> H\<tort_rbrace>") = \<open>K (NuSimpCong.simproc @{thm NuTopCtx_cong})\<close>
-
-lemma [\<nu>intro]: "\<^bold>c\<^bold>a\<^bold>s\<^bold>t h \<tycolon> H \<longmapsto> h' \<tycolon> H' \<^bold>w\<^bold>i\<^bold>t\<^bold>h Ph \<Longrightarrow>
-  \<^bold>c\<^bold>a\<^bold>s\<^bold>t s \<tycolon> S \<longmapsto> s' \<tycolon> S' \<^bold>w\<^bold>i\<^bold>t\<^bold>h Ps \<Longrightarrow>
-  \<^bold>c\<^bold>a\<^bold>s\<^bold>t (s \<tycolon> S\<heavy_comma> \<^bold>h\<^bold>e\<^bold>a\<^bold>p h \<tycolon> H) \<longmapsto> (s' \<tycolon> S'\<heavy_comma> \<^bold>h\<^bold>e\<^bold>a\<^bold>p h' \<tycolon> H') \<^bold>w\<^bold>i\<^bold>t\<^bold>h Ph \<and> Ps"
+lemma [\<nu>intro]: "\<^bold>c\<^bold>a\<^bold>s\<^bold>t H \<longmapsto> H' \<^bold>w\<^bold>i\<^bold>t\<^bold>h Ph \<Longrightarrow> \<^bold>c\<^bold>a\<^bold>s\<^bold>t S \<longmapsto> S' \<^bold>w\<^bold>i\<^bold>t\<^bold>h Ps \<Longrightarrow>
+  \<^bold>c\<^bold>a\<^bold>s\<^bold>t (S\<heavy_comma> \<^bold>h\<^bold>e\<^bold>a\<^bold>p H) \<longmapsto> (S'\<heavy_comma> \<^bold>h\<^bold>e\<^bold>a\<^bold>p H') \<^bold>w\<^bold>i\<^bold>t\<^bold>h Ph \<and> Ps"
   unfolding Cast_def by (simp add: nu_exps) blast
 
 subsection \<open>Fusion and its derivatives\<close>
@@ -506,33 +491,25 @@ term "\<tort_lbrace> a \<tycolon> A\<tort_rbrace> " *)
 
 subsubsection \<open>Stack Delimiter operator\<close>
 
-definition Stack_Delimiter :: "('a::lrep,'ax) \<nu> \<Rightarrow> ('b::lrep,'bx) \<nu> \<Rightarrow> ('a \<times> 'b, 'ax \<times> 'bx) \<nu>" (infixr "<stack-div>" 70)
-  where "A <stack-div> B = A \<cross_product> B"
-consts "Stack_Delimiter_sugar" :: " 'just \<Rightarrow> 'a \<Rightarrow> 'sugar " ( "_/ \<heavy_comma> _" [14,15] 14) \<comment> \<open>Note it is left associative\<close>
-translations " a \<tycolon> A\<heavy_comma> b \<tycolon> B " == " (CONST Pair b a) \<tycolon> (B <stack-div> A) "
-  " A \<heavy_comma> B" => " (CONST Pair (_\<nu>typing_x B) (_\<nu>typing_x A)) \<tycolon> ((_\<nu>typing_ty B) <stack-div> (_\<nu>typing_ty A)) "
+definition Stack_Delimiter :: " 'b::stack set \<Rightarrow> 'a::lrep set \<Rightarrow> ('a \<times> 'b) set" ( "_/ \<heavy_comma> _" [14,15] 14)
+  where "(B\<heavy_comma> A) = A \<times> B" \<comment> \<open>Note it is left associative\<close>
+translations " A\<heavy_comma> b \<tycolon> B " == "A\<heavy_comma> \<tort_lbrace>b \<tycolon> B\<tort_rbrace>"    " a \<tycolon> A\<heavy_comma> B " == "\<tort_lbrace>a \<tycolon> A\<tort_rbrace>\<heavy_comma> B"
 
-lemma [nu_exps]: "(pa,pb) \<nuLinkL> A <stack-div> B \<nuLinkR> (xa,xb) \<longleftrightarrow> (pa \<nuLinkL> A \<nuLinkR> xa) \<and> (pb \<nuLinkL> B \<nuLinkR> xb)"
-  unfolding Stack_Delimiter_def by (simp add: nu_exps)
-lemma [\<nu>elim,elim!]: "(a,b) \<ratio> A <stack-div> B \<Longrightarrow> (a \<ratio> A \<Longrightarrow> b \<ratio> B \<Longrightarrow> C) \<Longrightarrow> C"
-  unfolding Stack_Delimiter_def by blast
+lemma [nu_exps]: "(a,b) \<in> (B\<heavy_comma> A) \<longleftrightarrow> a \<in> A \<and> b \<in> B"
+  unfolding Stack_Delimiter_def by simp
+lemma [\<nu>elim,elim!]: "Inhabited (A\<heavy_comma> B) \<Longrightarrow> (Inhabited A \<Longrightarrow> Inhabited B \<Longrightarrow> C) \<Longrightarrow> C"
+  unfolding Stack_Delimiter_def Inhabited_def by blast
 
-lemma [\<nu>intro]: "\<^bold>c\<^bold>a\<^bold>s\<^bold>t a \<tycolon> A \<longmapsto> a' \<tycolon> A' \<^bold>w\<^bold>i\<^bold>t\<^bold>h P1 \<Longrightarrow> (P1 \<Longrightarrow> \<^bold>c\<^bold>a\<^bold>s\<^bold>t b \<tycolon> B \<longmapsto> b' \<tycolon> B' \<^bold>w\<^bold>i\<^bold>t\<^bold>h P2) \<Longrightarrow>
-  \<^bold>c\<^bold>a\<^bold>s\<^bold>t (a \<tycolon> A\<heavy_comma> b \<tycolon> B) \<longmapsto> (a' \<tycolon> A'\<heavy_comma> b' \<tycolon> B') \<^bold>w\<^bold>i\<^bold>t\<^bold>h P1 \<and> P2"
+lemma [\<nu>intro]: "\<^bold>c\<^bold>a\<^bold>s\<^bold>t A \<longmapsto> A' \<^bold>w\<^bold>i\<^bold>t\<^bold>h P1 \<Longrightarrow> (P1 \<Longrightarrow> \<^bold>c\<^bold>a\<^bold>s\<^bold>t B \<longmapsto> B' \<^bold>w\<^bold>i\<^bold>t\<^bold>h P2) \<Longrightarrow>
+  \<^bold>c\<^bold>a\<^bold>s\<^bold>t (A \<heavy_comma> B) \<longmapsto> (A'\<heavy_comma> B') \<^bold>w\<^bold>i\<^bold>t\<^bold>h P1 \<and> P2"
   unfolding Cast_def by (simp add: nu_exps) blast
-
-lemma Stack_Delimiter_cong: "\<tort_lbrace>a \<tycolon> A\<tort_rbrace> \<equiv> \<tort_lbrace>a' \<tycolon> A'\<tort_rbrace> \<Longrightarrow> \<tort_lbrace>b \<tycolon> B\<tort_rbrace> \<equiv> \<tort_lbrace>b' \<tycolon> B'\<tort_rbrace> \<Longrightarrow> \<tort_lbrace>b \<tycolon> B\<heavy_comma> a \<tycolon> A\<tort_rbrace> \<equiv> \<tort_lbrace>b' \<tycolon> B'\<heavy_comma> a' \<tycolon> A'\<tort_rbrace>"
-  unfolding atomize_eq by (auto 0 3 simp add: nu_exps)
-simproc_setup Stack_Delimiter_cong ("\<tort_lbrace>b \<tycolon> B\<heavy_comma> a \<tycolon> A\<tort_rbrace>") = \<open>K (NuSimpCong.simproc @{thm Stack_Delimiter_cong})\<close>
 
 subsubsection \<open>Front Stack\<close>
 
-definition Nu_Front_Stack :: "('a::lrep,'ax) \<nu> \<Rightarrow> (heap \<times> 'stack,'hsx) \<nu> \<Rightarrow> (heap \<times> 'a \<times> 'stack, 'ax \<times> 'hsx) \<nu>"
-  where "Nu_Front_Stack A Ctx = (\<lambda>(ax,hsx). {(h,a,s). (a \<nuLinkL> A \<nuLinkR> ax) \<and> ((h,s) \<nuLinkL> Ctx \<nuLinkR> (hsx))} )"
+definition Front_Stack :: " (heap \<times> 'stack) set \<Rightarrow> 'a set \<Rightarrow> (heap \<times> 'a \<times> 'stack) set" ( "_/ \<heavy_comma>^ _" [13,14] 13)
+  where "Front_Stack Ctx A = {(h,a,s). (h,s) \<in> Ctx \<and> a \<in> A}"
 
-consts "Front_Stack_sugar" :: " 'just \<Rightarrow> 'a \<Rightarrow> 'sugar " ( "_/ \<heavy_comma>^ _" [13,14] 13) \<comment> \<open>Note it is left associative\<close>
-translations " c \<tycolon> Ctx \<heavy_comma>^ a \<tycolon> A " == " (CONST Pair a c) \<tycolon> (CONST Nu_Front_Stack A Ctx) "
-  " Ctx \<heavy_comma>^ A " => " (CONST Pair (_\<nu>typing_x A) (_\<nu>typing_x Ctx)) \<tycolon> (CONST Nu_Front_Stack (_\<nu>typing_ty A) (_\<nu>typing_ty Ctx)) "
+translations " Ctx \<heavy_comma>^ a \<tycolon> A " == "Ctx \<heavy_comma>^ \<tort_lbrace>a \<tycolon> A\<tort_rbrace>"
 
 text \<open>Normally the stack elements are written `before` the heap elements, \<^term>\<open>s1 \<tycolon> S1\<heavy_comma> s2 \<tycolon> S2\<heavy_comma> \<^bold>h\<^bold>e\<^bold>a\<^bold>p h \<tycolon> H\<close>.
   The \<^term>\<open>Nu_Front_Stack\<close> allows one writes the stack elements `after` the heap, as \<^term>\<open>s1 \<tycolon> S1\<heavy_comma> \<^bold>h\<^bold>e\<^bold>a\<^bold>p h \<tycolon> H \<heavy_comma>^ s2 \<tycolon> S2\<close>.
@@ -541,28 +518,54 @@ text \<open>Normally the stack elements are written `before` the heap elements, 
     which requires body to return \<^term>\<open>x \<tycolon> X \<heavy_comma>^ loop_condition \<tycolon> Boolean\<close> where the \<^term>\<open>x \<tycolon> X\<close> instantiated by caller
     specifies all the heap and remaining stack except the leading loop_condition.\<close>
 
-lemma [nu_exps]: "(h,a,s) \<nuLinkL> Nu_Front_Stack A Ctx \<nuLinkR> (ax,hsx) \<longleftrightarrow> (a \<nuLinkL> A \<nuLinkR> ax) \<and> ((h,s) \<nuLinkL> Ctx \<nuLinkR> hsx)"
-  unfolding Nu_Front_Stack_def Refining_def by simp
-lemma [simp]: "\<tort_lbrace> (a,h,s) \<tycolon> Nu_Front_Stack A (NuTopCtx H S) \<tort_rbrace> = \<tort_lbrace> (h,a,s) \<tycolon> NuTopCtx H (A <stack-div> S) \<tort_rbrace>"
-  by (auto simp add: nu_exps)
+lemma [nu_exps]: "(h,a,s) \<in> (Ctx\<heavy_comma>^ A) \<longleftrightarrow> ((h,s) \<in> Ctx) \<and> (a \<in> A)"
+  unfolding Front_Stack_def by simp
+lemma [simp]: " (S\<heavy_comma> \<^bold>h\<^bold>e\<^bold>a\<^bold>p H \<heavy_comma>^ A) = (S\<heavy_comma> A\<heavy_comma> \<^bold>h\<^bold>e\<^bold>a\<^bold>p H) " by (auto simp add: nu_exps)
 
-lemma Nu_Front_Stack_cong: "\<tort_lbrace>c \<tycolon> Ctx\<tort_rbrace> \<equiv> \<tort_lbrace>c' \<tycolon> Ctx'\<tort_rbrace> \<Longrightarrow> \<tort_lbrace>c \<tycolon> Ctx \<heavy_comma>^ x \<tycolon> T\<tort_rbrace> \<equiv> \<tort_lbrace>c' \<tycolon> Ctx' \<heavy_comma>^ x \<tycolon> T\<tort_rbrace>"
-  unfolding atomize_eq by (auto simp add: nu_exps)
-simproc_setup Nu_Front_Stack_cong ("\<tort_lbrace>c \<tycolon> Ctx \<heavy_comma>^ x \<tycolon> T\<tort_rbrace>") = \<open>K (NuSimpCong.simproc @{thm Nu_Front_Stack_cong})\<close>
-
-lemma [\<nu>intro]: "\<^bold>c\<^bold>a\<^bold>s\<^bold>t R\<heavy_comma> \<^bold>h\<^bold>e\<^bold>a\<^bold>p H \<longmapsto> c \<tycolon> Ctx \<^bold>w\<^bold>i\<^bold>t\<^bold>h P \<Longrightarrow> \<^bold>i\<^bold>n\<^bold>t\<^bold>r\<^bold>o \<^bold>c\<^bold>a\<^bold>s\<^bold>t R\<heavy_comma> x \<tycolon> X\<heavy_comma> \<^bold>h\<^bold>e\<^bold>a\<^bold>p H \<longmapsto> c \<tycolon> Ctx \<heavy_comma>^ (x \<tycolon> X)"
+lemma [\<nu>intro]: "\<^bold>c\<^bold>a\<^bold>s\<^bold>t R\<heavy_comma> \<^bold>h\<^bold>e\<^bold>a\<^bold>p H \<longmapsto> Ctx \<^bold>w\<^bold>i\<^bold>t\<^bold>h P \<Longrightarrow> \<^bold>i\<^bold>n\<^bold>t\<^bold>r\<^bold>o \<^bold>c\<^bold>a\<^bold>s\<^bold>t R\<heavy_comma> x \<tycolon> X\<heavy_comma> \<^bold>h\<^bold>e\<^bold>a\<^bold>p H \<longmapsto> Ctx \<heavy_comma>^ (x \<tycolon> X)"
   unfolding Intro_def Cast_def by (simp add: nu_exps)
-lemma [\<nu>intro]: "\<^bold>c\<^bold>a\<^bold>s\<^bold>t c \<tycolon> Ctx \<longmapsto> (R\<heavy_comma> \<^bold>h\<^bold>e\<^bold>a\<^bold>p H) \<^bold>w\<^bold>i\<^bold>t\<^bold>h P
-    \<Longrightarrow> \<^bold>d\<^bold>e\<^bold>s\<^bold>t \<^bold>c\<^bold>a\<^bold>s\<^bold>t c \<tycolon> Ctx \<heavy_comma>^ (x \<tycolon> X) \<longmapsto> (R\<heavy_comma> x \<tycolon> X\<heavy_comma> \<^bold>h\<^bold>e\<^bold>a\<^bold>p H) \<^bold>w\<^bold>i\<^bold>t\<^bold>h P"
+lemma [\<nu>intro]: "\<^bold>c\<^bold>a\<^bold>s\<^bold>t Ctx \<longmapsto> (R\<heavy_comma> \<^bold>h\<^bold>e\<^bold>a\<^bold>p H) \<^bold>w\<^bold>i\<^bold>t\<^bold>h P
+    \<Longrightarrow> \<^bold>d\<^bold>e\<^bold>s\<^bold>t \<^bold>c\<^bold>a\<^bold>s\<^bold>t Ctx \<heavy_comma>^ (x \<tycolon> X) \<longmapsto> (R\<heavy_comma> x \<tycolon> X\<heavy_comma> \<^bold>h\<^bold>e\<^bold>a\<^bold>p H) \<^bold>w\<^bold>i\<^bold>t\<^bold>h P"
   unfolding Dest_def Cast_def by (simp add: nu_exps) blast
-lemma [\<nu>intro]: "\<^bold>c\<^bold>a\<^bold>s\<^bold>t x \<tycolon> X \<longmapsto> x' \<tycolon> X' \<^bold>w\<^bold>i\<^bold>t\<^bold>h Q \<Longrightarrow> \<^bold>c\<^bold>a\<^bold>s\<^bold>t R\<heavy_comma> \<^bold>h\<^bold>e\<^bold>a\<^bold>p H \<longmapsto> c \<tycolon> Ctx \<^bold>w\<^bold>i\<^bold>t\<^bold>h P
-  \<Longrightarrow> \<^bold>c\<^bold>a\<^bold>s\<^bold>t R\<heavy_comma> x \<tycolon> X\<heavy_comma> \<^bold>h\<^bold>e\<^bold>a\<^bold>p H \<longmapsto> c \<tycolon> Ctx \<heavy_comma>^ (x' \<tycolon> X') \<^bold>w\<^bold>i\<^bold>t\<^bold>h P \<and> Q"
+
+lemma [\<nu>intro 130]: "\<^bold>c\<^bold>a\<^bold>s\<^bold>t x \<tycolon> X \<longmapsto> x' \<tycolon> X' \<^bold>w\<^bold>i\<^bold>t\<^bold>h Q \<Longrightarrow> \<^bold>c\<^bold>a\<^bold>s\<^bold>t Ctx \<longmapsto> Ctx' \<^bold>w\<^bold>i\<^bold>t\<^bold>h P
+  \<Longrightarrow> \<^bold>c\<^bold>a\<^bold>s\<^bold>t Ctx \<heavy_comma>^ x \<tycolon> X \<longmapsto> Ctx' \<heavy_comma>^ (x' \<tycolon> X') \<^bold>w\<^bold>i\<^bold>t\<^bold>h P \<and> Q"
+  unfolding Cast_def by (simp add: nu_exps) blast
+
+lemma [\<nu>intro]: "\<^bold>c\<^bold>a\<^bold>s\<^bold>t x \<tycolon> X \<longmapsto> x' \<tycolon> X' \<^bold>w\<^bold>i\<^bold>t\<^bold>h Q \<Longrightarrow> \<^bold>c\<^bold>a\<^bold>s\<^bold>t R\<heavy_comma> \<^bold>h\<^bold>e\<^bold>a\<^bold>p H \<longmapsto> Ctx \<^bold>w\<^bold>i\<^bold>t\<^bold>h P
+  \<Longrightarrow> \<^bold>c\<^bold>a\<^bold>s\<^bold>t R\<heavy_comma> x \<tycolon> X\<heavy_comma> \<^bold>h\<^bold>e\<^bold>a\<^bold>p H \<longmapsto> Ctx \<heavy_comma>^ (x' \<tycolon> X') \<^bold>w\<^bold>i\<^bold>t\<^bold>h P \<and> Q"
+  unfolding Cast_def by (simp add: nu_exps) blast
+
+
+
+subsection \<open>Existential Nu-set\<close>
+
+definition ExSet :: " ('c \<Rightarrow> 'a set) \<Rightarrow> 'a set" (binder "\<exists>*" 10)
+  where "ExSet S = {p. (\<exists>c. p \<in> S c)}"
+notation ExSet (binder "\<exists>\<^sup>s" 10)
+
+lemma [simp]: "p \<in> ExSet S \<longleftrightarrow> (\<exists>c. p \<in> S c)" unfolding ExSet_def by simp
+
+lemma ExSet_pair: "ExSet T = (\<exists>*c1 c2. T (c1,c2) )" by (auto simp add: nu_exps)
+lemma named_ExSet: "(ExSet T) = (\<exists>*c. T (tag c) )" by (auto simp add: named_exists nu_exps)
+
+lemma [simp]: "p \<in> \<S>  (ExSet T) \<longleftrightarrow> (\<exists>z. p \<in> \<S>  (T z) )" by (auto 4 3 simp add: nu_exps)
+lemma [simp]: "p \<in> \<S_S> (ExSet T) \<longleftrightarrow> (\<exists>z. p \<in> \<S_S> (T z) )" by (auto 4 3 simp add: nu_exps)
+lemma [simp]: "(ExSet T \<heavy_comma> R) = (\<exists>* c. T c \<heavy_comma> R )" unfolding Stack_Delimiter_def by (auto simp add: nu_exps)
+lemma [simp]: "(L \<heavy_comma> ExSet T) = (\<exists>* c. L \<heavy_comma> T c )" unfolding Stack_Delimiter_def by (auto simp add: nu_exps)
+
+lemma ExTyp_strip: "(\<^bold>c\<^bold>u\<^bold>r\<^bold>r\<^bold>e\<^bold>n\<^bold>t p \<^bold>r\<^bold>e\<^bold>s\<^bold>u\<^bold>l\<^bold>t\<^bold>s \<^bold>i\<^bold>n (ExSet T)) \<equiv> (\<exists>c. \<^bold>c\<^bold>u\<^bold>r\<^bold>r\<^bold>e\<^bold>n\<^bold>t p \<^bold>r\<^bold>e\<^bold>s\<^bold>u\<^bold>l\<^bold>t\<^bold>s \<^bold>i\<^bold>n T c)"
+  unfolding CurrentConstruction_def by auto
+
+lemma ExTyp_I_\<nu>app[\<nu>intro 20]: "\<^bold>i\<^bold>n\<^bold>t\<^bold>r\<^bold>o \<^bold>c\<^bold>a\<^bold>s\<^bold>t T c \<longmapsto> (\<exists>*c. T c)"
+  unfolding Intro_def Cast_def by (simp add: nu_exps) blast
+lemma [\<nu>intro 200]: "(\<And>c. \<^bold>c\<^bold>a\<^bold>s\<^bold>t T c \<longmapsto> T' \<^bold>w\<^bold>i\<^bold>t\<^bold>h P c) \<Longrightarrow> \<^bold>c\<^bold>a\<^bold>s\<^bold>t (ExSet T) \<longmapsto> T' \<^bold>w\<^bold>i\<^bold>t\<^bold>h (\<exists>c. P c)"
   unfolding Cast_def by (simp add: nu_exps) blast
 
 
 
 
-subsection \<open>Existential Nu-type\<close>
+(* subsection \<open>Existential Nu-type\<close>
 
 definition ExNu :: " ('c \<Rightarrow> ('a,'b) \<nu>) \<Rightarrow> ('a, 'c \<Rightarrow> 'b) \<nu> "
   where "ExNu N x = {p. (\<exists>c. p \<nuLinkL> N c \<nuLinkR> x c)}"
@@ -617,7 +620,7 @@ lemma [simp]: "(ExTyp A \<heavy_comma> R) = (\<exists>* x. (A x \<heavy_comma> R
 lemma [simp]: "(S\<heavy_comma> ExTyp T) = (\<exists>* z. (S \<heavy_comma> T z))" by auto
 lemma ExTyp_strip: "(\<^bold>c\<^bold>u\<^bold>r\<^bold>r\<^bold>e\<^bold>n\<^bold>t p \<^bold>r\<^bold>e\<^bold>s\<^bold>u\<^bold>l\<^bold>t\<^bold>s \<^bold>i\<^bold>n (ExTyp T)) \<equiv> (\<exists>x. \<^bold>c\<^bold>u\<^bold>r\<^bold>r\<^bold>e\<^bold>n\<^bold>t p \<^bold>r\<^bold>e\<^bold>s\<^bold>u\<^bold>l\<^bold>t\<^bold>s \<^bold>i\<^bold>n T x)"
   unfolding CurrentConstruction_def by auto *)
-
+*)
 
 (* definition AutoExTyp :: "('a \<Rightarrow> 'b set) \<Rightarrow> 'b set" (binder "\<exists>*''" 10)
   where "AutoExTyp T = {x. (\<exists>z. x \<in> (T z))}"
@@ -632,7 +635,62 @@ lemma [simp]: "AutoExTyp T = (\<exists>*' a b. T (a,b))" unfolding AutoExTyp_def
 lemma AutoExTyp_strip: "(\<^bold>c\<^bold>u\<^bold>r\<^bold>r\<^bold>e\<^bold>n\<^bold>t p \<^bold>r\<^bold>e\<^bold>s\<^bold>u\<^bold>l\<^bold>t\<^bold>s \<^bold>i\<^bold>n (AutoExTyp T)) \<equiv> (\<exists>x. \<^bold>c\<^bold>u\<^bold>r\<^bold>r\<^bold>e\<^bold>n\<^bold>t p \<^bold>r\<^bold>e\<^bold>s\<^bold>u\<^bold>l\<^bold>t\<^bold>s \<^bold>i\<^bold>n T x)"
   unfolding AutoExTyp_def CurrentConstruction_def by (rule eq_reflection) auto *)
 
-subsection \<open>Addition Nu-type : coheres true proposition\<close>
+subsection \<open>Addition Nu-set : coheres true proposition\<close>
+
+definition AdditionSet :: " 'p set \<Rightarrow> bool \<Rightarrow> 'p set " (infixl "\<and>\<^sup>s" 35) where " (T \<and>\<^sup>s P) = {p. p \<in> T \<and> P}"
+translations "(x \<tycolon> T) \<and>\<^sup>s P" \<rightleftharpoons> "\<tort_lbrace>x \<tycolon> T\<tort_rbrace> \<and>\<^sup>s P"
+lemma [simp]: "p \<in> (T \<and>\<^sup>s P) \<longleftrightarrow> p \<in> T \<and> P" unfolding AdditionSet_def by simp
+
+lemma [\<nu>intro]: "\<^bold>p\<^bold>r\<^bold>e\<^bold>m\<^bold>i\<^bold>s\<^bold>e P \<Longrightarrow> \<^bold>i\<^bold>n\<^bold>t\<^bold>r\<^bold>o \<^bold>c\<^bold>a\<^bold>s\<^bold>t x \<tycolon> T \<longmapsto> (x \<tycolon> T) \<and>\<^sup>s P"
+  unfolding Intro_def Cast_def Premise_def by (simp add: nu_exps)
+lemma [\<nu>intro]: "\<^bold>c\<^bold>a\<^bold>s\<^bold>t T \<longmapsto> T' \<^bold>w\<^bold>i\<^bold>t\<^bold>h P \<Longrightarrow> \<^bold>p\<^bold>r\<^bold>e\<^bold>m\<^bold>i\<^bold>s\<^bold>e (P \<longrightarrow> Q) \<Longrightarrow> \<^bold>c\<^bold>a\<^bold>s\<^bold>t T \<longmapsto> T' \<and>\<^sup>s Q \<^bold>w\<^bold>i\<^bold>t\<^bold>h P"
+  unfolding Cast_def Premise_def by (simp add: nu_exps)
+
+lemma AdditionSet_simp_proc_arg[simp]: "\<^bold>p\<^bold>r\<^bold>o\<^bold>c f \<blangle> T \<and>\<^sup>s P \<longmapsto> Y \<brangle> = (P \<longrightarrow> \<^bold>p\<^bold>r\<^bold>o\<^bold>c f \<blangle> T \<longmapsto> Y \<brangle>)"
+  and AdditionSet_simp_func_arg[simp]: "\<^bold>f\<^bold>u\<^bold>n\<^bold>c f \<blangle> T \<and>\<^sup>s P \<longmapsto> Y \<brangle> = (P \<longrightarrow> \<^bold>f\<^bold>u\<^bold>n\<^bold>c f \<blangle> T \<longmapsto> Y \<brangle>)"
+  unfolding Auto_def Procedure_def Function_def by (simp add: nu_exps, blast)+
+
+lemma [simp]: "(T \<and>\<^sup>s True) = T" unfolding Auto_def by (auto simp add: nu_exps)
+lemma [simp]: "(L \<heavy_comma> T \<and>\<^sup>s P) = ((L \<heavy_comma> T) \<and>\<^sup>s P)"
+    and [simp]: "(T \<and>\<^sup>s P\<heavy_comma> R) = ((T\<heavy_comma> R) \<and>\<^sup>s P)"
+  unfolding Auto_def Stack_Delimiter_def by (auto simp add: nu_exps)
+lemma [simp]: "(L \<heavy_asterisk> (T \<and>\<^sup>s P)) = ((L \<heavy_asterisk> T) \<and>\<^sup>s P)"
+    and [simp]: "((T \<and>\<^sup>s P) \<heavy_asterisk> R) = ((T \<heavy_asterisk> R) \<and>\<^sup>s P)"
+  unfolding Auto_def Heap_Divider_def by (auto simp add: nu_exps) blast+
+lemma [simp]: "(S \<and>\<^sup>s P \<heavy_comma> \<^bold>h\<^bold>e\<^bold>a\<^bold>p H) = ((S\<heavy_comma> \<^bold>h\<^bold>e\<^bold>a\<^bold>p H) \<and>\<^sup>s P )"
+    and [simp]: "( S \<heavy_comma> \<^bold>h\<^bold>e\<^bold>a\<^bold>p H \<and>\<^sup>s P ) = ( (S\<heavy_comma> \<^bold>h\<^bold>e\<^bold>a\<^bold>p H) \<and>\<^sup>s P )"
+  unfolding Auto_def by (auto simp add: nu_exps)
+lemma [simp]: "( Ctx \<and>\<^sup>s P \<heavy_comma>^ T ) = ( (Ctx \<heavy_comma>^ T) \<and>\<^sup>s P ) "
+  unfolding Auto_def by (auto simp add: nu_exps)
+
+lemma [simp]: "(\<^bold>c\<^bold>u\<^bold>r\<^bold>r\<^bold>e\<^bold>n\<^bold>t s \<^bold>r\<^bold>e\<^bold>s\<^bold>u\<^bold>l\<^bold>t\<^bold>s \<^bold>i\<^bold>n T \<and>\<^sup>s P) \<longleftrightarrow> (\<^bold>c\<^bold>u\<^bold>r\<^bold>r\<^bold>e\<^bold>n\<^bold>t s \<^bold>r\<^bold>e\<^bold>s\<^bold>u\<^bold>l\<^bold>t\<^bold>s \<^bold>i\<^bold>n T) \<and> P"
+  unfolding CurrentConstruction_def Auto_def by (cases s) (simp add: nu_exps, blast+)
+lemma [simp]: "((\<^bold>c\<^bold>u\<^bold>r\<^bold>r\<^bold>e\<^bold>n\<^bold>t s \<^bold>r\<^bold>e\<^bold>s\<^bold>u\<^bold>l\<^bold>t\<^bold>s \<^bold>i\<^bold>n T) \<and> B) \<and> C \<longleftrightarrow> (\<^bold>c\<^bold>u\<^bold>r\<^bold>r\<^bold>e\<^bold>n\<^bold>t s \<^bold>r\<^bold>e\<^bold>s\<^bold>u\<^bold>l\<^bold>t\<^bold>s \<^bold>i\<^bold>n T) \<and> (B \<and> C)" by simp
+
+
+subsubsection \<open>Subj, the one cancelled the automatic discharging\<close>
+
+definition SetSubj :: " 'p set \<Rightarrow> bool \<Rightarrow> 'p set " (infixl "\<and>\<^sup>s\<^sup>!" 35) where " (\<and>\<^sup>s\<^sup>!) = (\<and>\<^sup>s)"
+
+lemma subj_\<nu>app: "\<^bold>p\<^bold>a\<^bold>r\<^bold>a\<^bold>m P \<Longrightarrow> \<^bold>p\<^bold>r\<^bold>e\<^bold>m\<^bold>i\<^bold>s\<^bold>e P \<Longrightarrow> \<^bold>c\<^bold>a\<^bold>s\<^bold>t T \<longmapsto> T \<and>\<^sup>s\<^sup>! P"
+  unfolding Cast_def Premise_def SetSubj_def by simp
+
+lemma [\<nu>intro]: "(P \<Longrightarrow> \<^bold>c\<^bold>a\<^bold>s\<^bold>t T \<longmapsto> T' \<^bold>w\<^bold>i\<^bold>t\<^bold>h Q) \<Longrightarrow> \<^bold>c\<^bold>a\<^bold>s\<^bold>t T \<and>\<^sup>s\<^sup>! P \<longmapsto> T' \<^bold>w\<^bold>i\<^bold>t\<^bold>h Q"
+  unfolding Cast_def SetSubj_def by simp blast
+lemma [\<nu>intro]: "\<^bold>c\<^bold>a\<^bold>s\<^bold>t T \<longmapsto> T' \<and>\<^sup>s P \<^bold>w\<^bold>i\<^bold>t\<^bold>h Q \<Longrightarrow> \<^bold>c\<^bold>a\<^bold>s\<^bold>t T \<longmapsto> T' \<and>\<^sup>s\<^sup>! P \<^bold>w\<^bold>i\<^bold>t\<^bold>h Q"
+  unfolding Cast_def SetSubj_def .
+
+
+(* lemma [simp]: "\<tort_lbrace> x \<tycolon> T \<and>\<^sup>\<nu> True\<tort_rbrace> = \<tort_lbrace> x \<tycolon> T \<tort_rbrace>" by auto
+lemma [simp]: "\<tort_lbrace>L \<heavy_comma> (x \<tycolon> T) \<and> P\<tort_rbrace> = \<tort_lbrace>(L \<heavy_comma> x \<tycolon> T) \<and> P\<tort_rbrace>" and [simp]: "\<tort_lbrace>(x \<tycolon> T) \<and> P\<heavy_comma> R\<tort_rbrace> = \<tort_lbrace>(x \<tycolon> T\<heavy_comma> R) \<and> P\<tort_rbrace>"
+  unfolding Stack_Delimiter_def by auto
+lemma [simp]: "\<tort_lbrace>L \<heavy_asterisk> (x \<tycolon> T) \<and> P\<tort_rbrace> = \<tort_lbrace>(L \<heavy_asterisk> x \<tycolon> T) \<and> P\<tort_rbrace>" and [simp]: "\<tort_lbrace>(x \<tycolon> T) \<and> P\<heavy_asterisk> R\<tort_rbrace> = \<tort_lbrace>(x \<tycolon> T\<heavy_asterisk> R) \<and> P\<tort_rbrace>"
+  unfolding Heap_Divider_def by auto blast+
+lemma [simp]: "\<tort_lbrace> (s \<tycolon> S) \<and> P \<heavy_comma> \<^bold>h\<^bold>e\<^bold>a\<^bold>p h \<tycolon> H \<tort_rbrace> = \<tort_lbrace> (s \<tycolon> S\<heavy_comma> \<^bold>h\<^bold>e\<^bold>a\<^bold>p h \<tycolon> H) \<and> P \<tort_rbrace>"
+  and [simp]: "\<tort_lbrace> s \<tycolon> S \<heavy_comma> \<^bold>h\<^bold>e\<^bold>a\<^bold>p (h \<tycolon> H) \<and> P \<tort_rbrace> = \<tort_lbrace> (s \<tycolon> S\<heavy_comma> \<^bold>h\<^bold>e\<^bold>a\<^bold>p h \<tycolon> H) \<and> P \<tort_rbrace>" by auto *)
+
+
+(* subsection \<open>Addition Nu-type : coheres true proposition\<close>
 
 definition NuAddition :: " ('p,'x) \<nu> \<Rightarrow> bool \<Rightarrow> ('p,'x) \<nu> " (infixl "\<and>\<^sup>\<nu>" 50)
   where " (N \<and>\<^sup>\<nu> P) = (\<lambda>x. {p. P \<and> (p \<nuLinkL> N \<nuLinkR> x)})"
@@ -652,56 +710,13 @@ lemma subj_\<nu>app: "\<^bold>p\<^bold>a\<^bold>r\<^bold>a\<^bold>m P \<Longrigh
 lemma [simp]: "\<tort_lbrace>L \<heavy_comma> (x \<tycolon> T) \<and> P\<tort_rbrace> = \<tort_lbrace>(L \<heavy_comma> x \<tycolon> T) \<and> P\<tort_rbrace>" and [simp]: "\<tort_lbrace>(x \<tycolon> T) \<and> P\<heavy_comma> R\<tort_rbrace> = \<tort_lbrace>(x \<tycolon> T\<heavy_comma> R) \<and> P\<tort_rbrace>"
   unfolding Stack_Delimiter_def by auto
 lemma [simp]: "\<tort_lbrace>L \<heavy_asterisk> (x \<tycolon> T) \<and> P\<tort_rbrace> = \<tort_lbrace>(L \<heavy_asterisk> x \<tycolon> T) \<and> P\<tort_rbrace>" and [simp]: "\<tort_lbrace>(x \<tycolon> T) \<and> P\<heavy_asterisk> R\<tort_rbrace> = \<tort_lbrace>(x \<tycolon> T\<heavy_asterisk> R) \<and> P\<tort_rbrace>"
-  unfolding Heap_Delimiter_def by auto blast+
+  unfolding Heap_Divider_def by auto blast+
 lemma [simp]: "\<tort_lbrace> (s \<tycolon> S) \<and> P \<heavy_comma> \<^bold>h\<^bold>e\<^bold>a\<^bold>p h \<tycolon> H \<tort_rbrace> = \<tort_lbrace> (s \<tycolon> S\<heavy_comma> \<^bold>h\<^bold>e\<^bold>a\<^bold>p h \<tycolon> H) \<and> P \<tort_rbrace>"
   and [simp]: "\<tort_lbrace> s \<tycolon> S \<heavy_comma> \<^bold>h\<^bold>e\<^bold>a\<^bold>p (h \<tycolon> H) \<and> P \<tort_rbrace> = \<tort_lbrace> (s \<tycolon> S\<heavy_comma> \<^bold>h\<^bold>e\<^bold>a\<^bold>p h \<tycolon> H) \<and> P \<tort_rbrace>" by auto *)
 
 lemma NuAddition_cong: "\<tort_lbrace>x \<tycolon> T\<tort_rbrace> \<equiv> \<tort_lbrace>x' \<tycolon> T'\<tort_rbrace> \<Longrightarrow> \<tort_lbrace>x \<tycolon> T \<and>\<^sup>\<nu> P\<tort_rbrace> \<equiv> \<tort_lbrace>x' \<tycolon> T' \<and>\<^sup>\<nu> P\<tort_rbrace>" unfolding atomize_eq by (auto simp add: nu_exps)
 simproc_setup NuAddition_cong ("\<tort_lbrace>x \<tycolon> T \<and>\<^sup>\<nu> P\<tort_rbrace>") = \<open>K (NuSimpCong.simproc @{thm NuAddition_cong})\<close>
-
-subsubsection \<open>Auto tag\<close>
-
-abbreviation AutoAddition (infixl "\<and>\<^sup>\<nu>''" 50) where "AutoAddition T P \<equiv> Auto (NuAddition T P)"
-notation AutoAddition (infixl "\<and>\<^sup>\<nu>\<^sub>a\<^sub>u\<^sub>t\<^sub>o" 50)
-translations "(x \<tycolon> T) \<and>\<^sup>\<nu>\<^sub>a\<^sub>u\<^sub>t\<^sub>o P" \<rightleftharpoons> "x \<tycolon> T \<and>\<^sup>\<nu>\<^sub>a\<^sub>u\<^sub>t\<^sub>o P"
-
-lemma [simp]: "\<^bold>p\<^bold>r\<^bold>o\<^bold>c f \<blangle> x \<tycolon> T \<and>\<^sup>\<nu>\<^sub>a\<^sub>u\<^sub>t\<^sub>o P \<longmapsto> Y \<brangle> = (P \<longrightarrow> \<^bold>p\<^bold>r\<^bold>o\<^bold>c f \<blangle> x \<tycolon> T \<longmapsto> Y \<brangle>)"
-  unfolding Auto_def Procedure_def by (simp add: nu_exps) blast
-lemma [simp]: "\<^bold>p\<^bold>r\<^bold>o\<^bold>c f \<blangle> X \<longmapsto> y \<tycolon> Y \<and>\<^sup>\<nu>\<^sub>a\<^sub>u\<^sub>t\<^sub>o P \<brangle> = \<^bold>p\<^bold>r\<^bold>o\<^bold>c f \<blangle> X \<longmapsto> y \<tycolon> Y \<and>\<^sup>\<nu> P \<brangle>"
-  unfolding Auto_def ..
-lemma [simp]: "\<^bold>f\<^bold>u\<^bold>n\<^bold>c f \<blangle> x \<tycolon> T \<and>\<^sup>\<nu>\<^sub>a\<^sub>u\<^sub>t\<^sub>o P \<longmapsto> Y \<brangle> = (P \<longrightarrow> \<^bold>f\<^bold>u\<^bold>n\<^bold>c f \<blangle> x \<tycolon> T \<longmapsto> Y \<brangle>)"
-  unfolding Function_def by simp
-lemma [simp]: "\<^bold>f\<^bold>u\<^bold>n\<^bold>c f \<blangle> X \<longmapsto> y \<tycolon> Y \<and>\<^sup>\<nu>\<^sub>a\<^sub>u\<^sub>t\<^sub>o P \<brangle> = \<^bold>f\<^bold>u\<^bold>n\<^bold>c f \<blangle> X \<longmapsto> y \<tycolon> Y \<and>\<^sup>\<nu> P \<brangle>"
-  unfolding Auto_def ..
-
-
-lemma [simp]: "\<tort_lbrace> x \<tycolon> T \<and>\<^sup>\<nu>\<^sub>a\<^sub>u\<^sub>t\<^sub>o True\<tort_rbrace> = \<tort_lbrace> x \<tycolon> T \<tort_rbrace>" unfolding Auto_def by (auto simp add: nu_exps)
-lemma [simp]: "\<tort_lbrace>L \<heavy_comma> (x \<tycolon> T) \<and>\<^sup>\<nu>\<^sub>a\<^sub>u\<^sub>t\<^sub>o P\<tort_rbrace> = \<tort_lbrace>(L \<heavy_comma> x \<tycolon> T) \<and>\<^sup>\<nu>\<^sub>a\<^sub>u\<^sub>t\<^sub>o P\<tort_rbrace>"
-    and [simp]: "\<tort_lbrace>(x \<tycolon> T) \<and>\<^sup>\<nu>\<^sub>a\<^sub>u\<^sub>t\<^sub>o P\<heavy_comma> R\<tort_rbrace> = \<tort_lbrace>(x \<tycolon> T\<heavy_comma> R) \<and>\<^sup>\<nu>\<^sub>a\<^sub>u\<^sub>t\<^sub>o P\<tort_rbrace>"
-  unfolding Auto_def Stack_Delimiter_def by (auto simp add: nu_exps)
-lemma [simp]: "\<tort_lbrace>L \<heavy_asterisk> (x \<tycolon> T) \<and>\<^sup>\<nu>\<^sub>a\<^sub>u\<^sub>t\<^sub>o P\<tort_rbrace> = \<tort_lbrace>(L \<heavy_asterisk> x \<tycolon> T) \<and>\<^sup>\<nu>\<^sub>a\<^sub>u\<^sub>t\<^sub>o P\<tort_rbrace>"
-    and [simp]: "\<tort_lbrace>(x \<tycolon> T) \<and>\<^sup>\<nu>\<^sub>a\<^sub>u\<^sub>t\<^sub>o P \<heavy_asterisk> R\<tort_rbrace> = \<tort_lbrace>(x \<tycolon> T\<heavy_asterisk> R) \<and>\<^sup>\<nu>\<^sub>a\<^sub>u\<^sub>t\<^sub>o P\<tort_rbrace>"
-  unfolding Auto_def Heap_Delimiter_def by (auto simp add: nu_exps) blast+
-lemma [simp]: "\<tort_lbrace> (s \<tycolon> S) \<and>\<^sup>\<nu>\<^sub>a\<^sub>u\<^sub>t\<^sub>o P \<heavy_comma> \<^bold>h\<^bold>e\<^bold>a\<^bold>p h \<tycolon> H \<tort_rbrace> = \<tort_lbrace> (s \<tycolon> S\<heavy_comma> \<^bold>h\<^bold>e\<^bold>a\<^bold>p h \<tycolon> H) \<and>\<^sup>\<nu>\<^sub>a\<^sub>u\<^sub>t\<^sub>o P \<tort_rbrace>"
-    and [simp]: "\<tort_lbrace> s \<tycolon> S \<heavy_comma> \<^bold>h\<^bold>e\<^bold>a\<^bold>p (h \<tycolon> H) \<and>\<^sup>\<nu>\<^sub>a\<^sub>u\<^sub>t\<^sub>o P \<tort_rbrace> = \<tort_lbrace> (s \<tycolon> S\<heavy_comma> \<^bold>h\<^bold>e\<^bold>a\<^bold>p h \<tycolon> H) \<and>\<^sup>\<nu>\<^sub>a\<^sub>u\<^sub>t\<^sub>o P \<tort_rbrace>"
-  unfolding Auto_def by (auto simp add: nu_exps)
-lemma [simp]: "\<tort_lbrace>c \<tycolon> Ctx \<and>\<^sup>\<nu>\<^sub>a\<^sub>u\<^sub>t\<^sub>o P \<heavy_comma>^ x \<tycolon> T\<tort_rbrace> = \<tort_lbrace> (c \<tycolon> Ctx \<heavy_comma>^ x \<tycolon> T) \<and>\<^sup>\<nu>\<^sub>a\<^sub>u\<^sub>t\<^sub>o P \<tort_rbrace>"
-  unfolding Auto_def by (auto simp add: nu_exps)
-
-lemma AutoAddition_cong: "\<tort_lbrace>x \<tycolon> T\<tort_rbrace> \<equiv> \<tort_lbrace>x' \<tycolon> T'\<tort_rbrace> \<Longrightarrow> \<tort_lbrace>x \<tycolon> T \<and>\<^sup>\<nu>\<^sub>a\<^sub>u\<^sub>t\<^sub>o P\<tort_rbrace> \<equiv> \<tort_lbrace>x' \<tycolon> T' \<and>\<^sup>\<nu>\<^sub>a\<^sub>u\<^sub>t\<^sub>o P\<tort_rbrace>" unfolding Auto_def by simp
-simproc_setup AutoAddition_cong ("\<tort_lbrace>x \<tycolon> T \<and>\<^sup>\<nu>\<^sub>a\<^sub>u\<^sub>t\<^sub>o P\<tort_rbrace>") = \<open>K (NuSimpCong.simproc @{thm AutoAddition_cong})\<close>
-
-lemma t1: "(\<^bold>c\<^bold>u\<^bold>r\<^bold>r\<^bold>e\<^bold>n\<^bold>t s \<^bold>r\<^bold>e\<^bold>s\<^bold>u\<^bold>l\<^bold>t\<^bold>s \<^bold>i\<^bold>n (x \<tycolon> T) \<and>\<^sup>\<nu>\<^sub>a\<^sub>u\<^sub>t\<^sub>o P) \<longleftrightarrow> (\<^bold>c\<^bold>u\<^bold>r\<^bold>r\<^bold>e\<^bold>n\<^bold>t s \<^bold>r\<^bold>e\<^bold>s\<^bold>u\<^bold>l\<^bold>t\<^bold>s \<^bold>i\<^bold>n x \<tycolon> T) \<and> P"
-  unfolding CurrentConstruction_def Auto_def by (cases s) (simp add: nu_exps, blast+)
-lemma [simp]: "((((\<^bold>c\<^bold>u\<^bold>r\<^bold>r\<^bold>e\<^bold>n\<^bold>t s \<^bold>r\<^bold>e\<^bold>s\<^bold>u\<^bold>l\<^bold>t\<^bold>s \<^bold>i\<^bold>n T) \<and> B) \<and> C) \<^bold>w\<^bold>i\<^bold>t\<^bold>h \<^bold>f\<^bold>a\<^bold>c\<^bold>t\<^bold>s: PROP L) \<equiv> (((\<^bold>c\<^bold>u\<^bold>r\<^bold>r\<^bold>e\<^bold>n\<^bold>t s \<^bold>r\<^bold>e\<^bold>s\<^bold>u\<^bold>l\<^bold>t\<^bold>s \<^bold>i\<^bold>n T) \<and> (B \<and> C)) \<^bold>w\<^bold>i\<^bold>t\<^bold>h \<^bold>f\<^bold>a\<^bold>c\<^bold>t\<^bold>s: PROP L)" by simp
-
-lemma extract_addition_fact_major:
-  "(\<^bold>c\<^bold>u\<^bold>r\<^bold>r\<^bold>e\<^bold>n\<^bold>t s \<^bold>r\<^bold>e\<^bold>s\<^bold>u\<^bold>l\<^bold>t\<^bold>s \<^bold>i\<^bold>n (x \<tycolon> T) \<and>\<^sup>\<nu>\<^sub>a\<^sub>u\<^sub>t\<^sub>o Q) \<Longrightarrow> (\<^bold>c\<^bold>u\<^bold>r\<^bold>r\<^bold>e\<^bold>n\<^bold>t s \<^bold>r\<^bold>e\<^bold>s\<^bold>u\<^bold>l\<^bold>t\<^bold>s \<^bold>i\<^bold>n (x \<tycolon> T))"
-  by (meson CurrentConstruction_def t1)
-lemma extract_addition_fact_minor:
-  "(\<^bold>c\<^bold>u\<^bold>r\<^bold>r\<^bold>e\<^bold>n\<^bold>t s \<^bold>r\<^bold>e\<^bold>s\<^bold>u\<^bold>l\<^bold>t\<^bold>s \<^bold>i\<^bold>n (x \<tycolon> T) \<and>\<^sup>\<nu>\<^sub>a\<^sub>u\<^sub>t\<^sub>o Q) \<Longrightarrow> Q"
-  by (meson CurrentConstruction_def t1)
-
+*)
 
 subsection \<open>Identity\<close>
 
@@ -729,7 +744,7 @@ lemma refine_\<nu>app: "\<^bold>p\<^bold>a\<^bold>r\<^bold>a\<^bold>m P \<Longri
 
 abbreviation AutoRefine (infixl "<auto-where>" 80)
   where "AutoRefine N P \<equiv> Auto (NuRefine N P)"
-lemma [simp]:"\<tort_lbrace>x \<tycolon> T <auto-where> P \<tort_rbrace> = \<tort_lbrace> (x \<tycolon> T) \<and>\<^sup>\<nu>\<^sub>a\<^sub>u\<^sub>t\<^sub>o (\<^bold>p\<^bold>r\<^bold>e\<^bold>m\<^bold>i\<^bold>s\<^bold>e x \<in> P) \<tort_rbrace>"
+lemma [simp]:"\<tort_lbrace>x \<tycolon> T <auto-where> P \<tort_rbrace> = ((x \<tycolon> T) \<and>\<^sup>s (\<^bold>p\<^bold>r\<^bold>e\<^bold>m\<^bold>i\<^bold>s\<^bold>e x \<in> P))"
   unfolding Auto_def Premise_def by (auto simp add: nu_exps)
 
 lemma NuRefine_to_auto:"\<tort_lbrace>x \<tycolon> T <where> P \<tort_rbrace> = \<tort_lbrace>x \<tycolon> T <auto-where> P \<tort_rbrace>" unfolding Auto_def ..
@@ -812,7 +827,9 @@ lemma [\<nu>intro 130]: "\<^bold>c\<^bold>a\<^bold>s\<^bold>t x \<tycolon> M \<l
   unfolding Dest_def Cast_def CaseSplit_def by auto *)
 lemma [\<nu>intro 20]: "(\<And> x. y = g x \<Longrightarrow> \<^bold>c\<^bold>a\<^bold>s\<^bold>t x \<tycolon> M \<longmapsto> N \<^bold>w\<^bold>i\<^bold>t\<^bold>h P x) \<Longrightarrow> \<^bold>c\<^bold>a\<^bold>s\<^bold>t y \<tycolon> M <up-lift> g \<longmapsto> N \<^bold>w\<^bold>i\<^bold>t\<^bold>h (\<exists>x. y = g x \<and> P x)"
   unfolding Dest_def Cast_def CaseSplit_def by (simp add: nu_exps) blast
-lemma [\<nu>intro 150]: "(\<And> x. y = g x \<Longrightarrow> \<^bold>c\<^bold>a\<^bold>s\<^bold>t x \<tycolon> M \<longmapsto> y' x \<tycolon> M' x \<^bold>w\<^bold>i\<^bold>t\<^bold>h P x) \<Longrightarrow> \<^bold>c\<^bold>a\<^bold>s\<^bold>t y \<tycolon> M <up-lift> g \<longmapsto>( \<exists>*x. y' x \<tycolon> M' x) \<^bold>w\<^bold>i\<^bold>t\<^bold>h (\<exists>x. y = g x \<and> P x)"
+lemma [\<nu>intro 150]:
+  "(\<And> x. y = g x \<Longrightarrow> \<^bold>c\<^bold>a\<^bold>s\<^bold>t x \<tycolon> M \<longmapsto> y' x \<tycolon> M' x \<^bold>w\<^bold>i\<^bold>t\<^bold>h P x)
+    \<Longrightarrow> \<^bold>c\<^bold>a\<^bold>s\<^bold>t y \<tycolon> M <up-lift> g \<longmapsto> (\<exists>*x. \<tort_lbrace>y' x \<tycolon> M' x\<tort_rbrace> ) \<^bold>w\<^bold>i\<^bold>t\<^bold>h (\<exists>x. y = g x \<and> P x)"
   unfolding Dest_def Cast_def CaseSplit_def by (simp add: nu_exps) blast
 
 (*term case_prod
@@ -834,8 +851,8 @@ val th'2 = REPEAT (eresolve0_tac @{thms A} 1
 thm if_split
 thm prod.split_asm
 *)
-lemma "\<^bold>d\<^bold>e\<^bold>s\<^bold>t \<^bold>c\<^bold>a\<^bold>s\<^bold>t y \<tycolon> M <up-lift> g \<longmapsto> (\<exists>* x. x \<tycolon> M \<and>\<^sup>\<nu> (g x = y))"
-  unfolding Dest_def Cast_def by (simp add: nu_exps)
+lemma "\<^bold>d\<^bold>e\<^bold>s\<^bold>t \<^bold>c\<^bold>a\<^bold>s\<^bold>t y \<tycolon> M <up-lift> g \<longmapsto> (\<exists>* x. (x \<tycolon> M) \<and>\<^sup>s g x = y)"
+  unfolding Dest_def Cast_def by (simp add: nu_exps) blast
 
 lemma "\<^bold>c\<^bold>a\<^bold>s\<^bold>t x \<tycolon> N \<longmapsto> f x \<tycolon> N <up-lift> f" unfolding Cast_def by (simp add: nu_exps) blast
 lemma "\<^bold>c\<^bold>a\<^bold>s\<^bold>t x \<tycolon> N \<longmapsto> f x \<tycolon> N <up-lift> f" unfolding Cast_def by (simp add: nu_exps) blast
@@ -858,17 +875,18 @@ lemma [\<nu>intro]: "\<^bold>c\<^bold>a\<^bold>s\<^bold>t x \<tycolon> N \<longm
 lemma someE_\<nu>cast[\<nu>cast_overload E]: "[h] \<^bold>c\<^bold>a\<^bold>s\<^bold>t X \<tycolon> (\<^bold>s\<^bold>o\<^bold>m\<^bold>e N) \<longmapsto> (\<exists>*some. \<tort_lbrace>some \<tycolon> N \<tort_rbrace> \<addition> (some \<in> X))" unfolding Cast_def by auto *)
 
 
-section \<open>Mechanisms - II\<close>
+section \<open>Mechanisms - II - Main Parts\<close>
 
 subsection \<open>Heap\<close>
 
-definition NuNothing :: "(heap, unit) \<nu>" where  "NuNothing x = {h. h = Map.empty}"
+abbreviation Nothing :: "heap set" where "Nothing \<equiv> {Map.empty}"
+(* definition NuNothing :: "(heap, unit) \<nu>" where  "NuNothing x = {h. h = Map.empty}"
 consts Nothing_sugar :: " 'a_sugar " ("Nothing")
 translations "Nothing" \<rightleftharpoons> "() \<tycolon> CONST NuNothing"
-lemma [nu_exps]: "h \<nuLinkL> NuNothing \<nuLinkR> x \<longleftrightarrow> h = Map.empty" unfolding Refining_def NuNothing_def by simp
+lemma [nu_exps]: "h \<nuLinkL> NuNothing \<nuLinkR> x \<longleftrightarrow> h = Map.empty" unfolding Refining_def NuNothing_def by simp *)
 
-lemma Separation_emptyL: "\<tort_lbrace>Nothing \<heavy_asterisk> h \<tycolon> H\<tort_rbrace> = \<tort_lbrace>h \<tycolon> H\<tort_rbrace>" and Separation_emptyR: "\<tort_lbrace>h \<tycolon> H \<heavy_asterisk> Nothing\<tort_rbrace> = \<tort_lbrace>h \<tycolon> H\<tort_rbrace>"
-  unfolding Heap_Delimiter_def by (auto simp add: nu_exps)
+lemma Separation_emptyL[simp]: "(Nothing \<heavy_asterisk> H) = H" and Separation_emptyR[simp]: "(H \<heavy_asterisk> Nothing) = H"
+  unfolding Heap_Divider_def by (auto simp add: nu_exps)
 
 subsubsection \<open>Syntax & Auxiliary\<close>
 
@@ -933,19 +951,18 @@ subsubsection \<open>Cast\<close>
 
 definition Heap_Cast_Goal :: " 'a \<Rightarrow> 'a "  ("\<medium_left_bracket>\<medium_left_bracket> _ \<medium_right_bracket>\<medium_right_bracket>") where "Heap_Cast_Goal x = x"
   \<comment> \<open>The protector marks the goal to be gained\<close>
+translations "\<medium_left_bracket>\<medium_left_bracket> x \<tycolon> T \<medium_right_bracket>\<medium_right_bracket>" \<rightleftharpoons> " \<medium_left_bracket>\<medium_left_bracket> \<tort_lbrace>x \<tycolon> T\<tort_rbrace> \<medium_right_bracket>\<medium_right_bracket> "
 
-lemma [\<nu>intro 1000]: "\<medium_left_bracket>\<medium_left_bracket> \<^bold>c\<^bold>a\<^bold>s\<^bold>t h \<tycolon> H \<longmapsto> h \<tycolon> \<medium_left_bracket>\<medium_left_bracket> H \<medium_right_bracket>\<medium_right_bracket> \<^bold>d\<^bold>u\<^bold>a\<^bold>l h\<^sub>m \<tycolon> \<medium_left_bracket>\<medium_left_bracket> H\<^sub>m \<medium_right_bracket>\<medium_right_bracket> \<longmapsto> h\<^sub>m \<tycolon> H\<^sub>m \<medium_right_bracket>\<medium_right_bracket>" unfolding Heap_Cast_Goal_def using cast_dual_id .
-
-lemma context_cast[\<nu>intro]:
-  "\<^bold>c\<^bold>a\<^bold>s\<^bold>t k \<tycolon> K \<longmapsto> k' \<tycolon> K' \<^bold>w\<^bold>i\<^bold>t\<^bold>h P \<Longrightarrow>
-   \<medium_left_bracket>\<medium_left_bracket> \<^bold>c\<^bold>a\<^bold>s\<^bold>t h \<tycolon> H \<longmapsto> h' \<tycolon> \<medium_left_bracket>\<medium_left_bracket> H' \<medium_right_bracket>\<medium_right_bracket> \<^bold>w\<^bold>i\<^bold>t\<^bold>h Q \<medium_right_bracket>\<medium_right_bracket> \<Longrightarrow>
-   \<^bold>c\<^bold>a\<^bold>s\<^bold>t (k \<tycolon> K\<heavy_comma> \<^bold>h\<^bold>e\<^bold>a\<^bold>p h \<tycolon> H) \<longmapsto> (k' \<tycolon> K'\<heavy_comma> \<^bold>h\<^bold>e\<^bold>a\<^bold>p h' \<tycolon> H') \<^bold>w\<^bold>i\<^bold>t\<^bold>h P \<and> Q"
+lemma context_cast[\<nu>intro 1000]:
+  "\<^bold>c\<^bold>a\<^bold>s\<^bold>t K \<longmapsto> K' \<^bold>w\<^bold>i\<^bold>t\<^bold>h P \<Longrightarrow>
+   \<medium_left_bracket>\<medium_left_bracket> \<^bold>c\<^bold>a\<^bold>s\<^bold>t H \<longmapsto> \<medium_left_bracket>\<medium_left_bracket> H' \<medium_right_bracket>\<medium_right_bracket> \<^bold>w\<^bold>i\<^bold>t\<^bold>h Q \<medium_right_bracket>\<medium_right_bracket> \<Longrightarrow>
+   \<^bold>c\<^bold>a\<^bold>s\<^bold>t (K\<heavy_comma> \<^bold>h\<^bold>e\<^bold>a\<^bold>p H) \<longmapsto> (K'\<heavy_comma> \<^bold>h\<^bold>e\<^bold>a\<^bold>p H') \<^bold>w\<^bold>i\<^bold>t\<^bold>h P \<and> Q"
   unfolding Cast_def Heap_Cast_Goal_def by (simp add: pair_forall nu_exps) blast
 
-lemma context_cast_dual[\<nu>intro]:
-  "\<^bold>c\<^bold>a\<^bold>s\<^bold>t k \<tycolon> K \<longmapsto> k' \<tycolon> K' \<^bold>w\<^bold>i\<^bold>t\<^bold>h PK
-    \<Longrightarrow> (PK \<Longrightarrow> \<medium_left_bracket>\<medium_left_bracket> \<^bold>c\<^bold>a\<^bold>s\<^bold>t h \<tycolon> H \<longmapsto> h' \<tycolon> \<medium_left_bracket>\<medium_left_bracket> H' \<medium_right_bracket>\<medium_right_bracket> \<^bold>w\<^bold>i\<^bold>t\<^bold>h PH \<^bold>d\<^bold>u\<^bold>a\<^bold>l h2 \<tycolon> \<medium_left_bracket>\<medium_left_bracket> H2 \<medium_right_bracket>\<medium_right_bracket> \<longmapsto> h2' \<tycolon> H2' \<medium_right_bracket>\<medium_right_bracket>)
-    \<Longrightarrow> \<^bold>c\<^bold>a\<^bold>s\<^bold>t (k \<tycolon> K\<heavy_comma> \<^bold>h\<^bold>e\<^bold>a\<^bold>p h \<tycolon> H) \<longmapsto> (k' \<tycolon> K'\<heavy_comma> \<^bold>h\<^bold>e\<^bold>a\<^bold>p h' \<tycolon> H') \<^bold>w\<^bold>i\<^bold>t\<^bold>h PK \<and> PH \<^bold>d\<^bold>u\<^bold>a\<^bold>l (k2 \<tycolon> K2\<heavy_comma> \<^bold>h\<^bold>e\<^bold>a\<^bold>p h2 \<tycolon> H2) \<longmapsto> (k2 \<tycolon> K2\<heavy_comma> \<^bold>h\<^bold>e\<^bold>a\<^bold>p h2' \<tycolon> H2')"
+lemma context_cast_dual[\<nu>intro 1000]:
+  "\<^bold>c\<^bold>a\<^bold>s\<^bold>t K \<longmapsto> K' \<^bold>w\<^bold>i\<^bold>t\<^bold>h PK
+    \<Longrightarrow> (PK \<Longrightarrow> \<medium_left_bracket>\<medium_left_bracket> \<^bold>c\<^bold>a\<^bold>s\<^bold>t H \<longmapsto> \<medium_left_bracket>\<medium_left_bracket> H' \<medium_right_bracket>\<medium_right_bracket> \<^bold>w\<^bold>i\<^bold>t\<^bold>h PH \<^bold>d\<^bold>u\<^bold>a\<^bold>l \<medium_left_bracket>\<medium_left_bracket> H2 \<medium_right_bracket>\<medium_right_bracket> \<longmapsto> H2' \<medium_right_bracket>\<medium_right_bracket>)
+    \<Longrightarrow> \<^bold>c\<^bold>a\<^bold>s\<^bold>t (K\<heavy_comma> \<^bold>h\<^bold>e\<^bold>a\<^bold>p H) \<longmapsto> (K'\<heavy_comma> \<^bold>h\<^bold>e\<^bold>a\<^bold>p H') \<^bold>w\<^bold>i\<^bold>t\<^bold>h PK \<and> PH \<^bold>d\<^bold>u\<^bold>a\<^bold>l (K2\<heavy_comma> \<^bold>h\<^bold>e\<^bold>a\<^bold>p H2) \<longmapsto> (K2\<heavy_comma> \<^bold>h\<^bold>e\<^bold>a\<^bold>p H2')"
   unfolding CastDual_def Cast_def Heap_Cast_Goal_def Intro_def Dest_def by (simp add: pair_forall nu_exps) blast
 
 (* lemma [\<nu>intro0]: "\<^bold>c\<^bold>a\<^bold>s\<^bold>t x \<tycolon> X \<longmapsto> H' \<heavy_asterisk> y \<tycolon> Y \<^bold>w\<^bold>i\<^bold>t\<^bold>h P \<^bold>d\<^bold>u\<^bold>a\<^bold>l H'\<^sub>m \<heavy_asterisk> y\<^sub>m \<tycolon> Y \<longmapsto> x\<^sub>m \<tycolon> X \<^bold>w\<^bold>h\<^bold>e\<^bold>n Q
@@ -953,81 +970,101 @@ lemma context_cast_dual[\<nu>intro]:
   unfolding Heap_Cast_Goal_def . *)
 (* lemma [\<nu>intro0]: "\<^bold>c\<^bold>a\<^bold>s\<^bold>t A \<longmapsto> A \<^bold>d\<^bold>u\<^bold>a\<^bold>l B \<longmapsto> B" unfolding CastDual_def  by (simp add: cast_id) *)
 
-lemma [\<nu>intro 1000]:
-  "\<medium_left_bracket>\<medium_left_bracket> \<^bold>c\<^bold>a\<^bold>s\<^bold>t L \<heavy_asterisk> h \<tycolon> H \<longmapsto> L \<heavy_asterisk> h \<tycolon> \<medium_left_bracket>\<medium_left_bracket> H \<medium_right_bracket>\<medium_right_bracket> \<^bold>d\<^bold>u\<^bold>a\<^bold>l L \<heavy_asterisk> h\<^sub>m \<tycolon> \<medium_left_bracket>\<medium_left_bracket> H\<^sub>m \<medium_right_bracket>\<medium_right_bracket> \<longmapsto> L \<heavy_asterisk> h\<^sub>m \<tycolon> H\<^sub>m \<medium_right_bracket>\<medium_right_bracket>"
-  unfolding Heap_Cast_Goal_def using cast_dual_id .
+(* lemma [\<nu>intro 1000]:
+  "\<medium_left_bracket>\<medium_left_bracket> \<^bold>c\<^bold>a\<^bold>s\<^bold>t L \<heavy_asterisk> H \<longmapsto> L \<heavy_asterisk> H \<^bold>d\<^bold>u\<^bold>a\<^bold>l L \<heavy_asterisk> h\<^sub>m \<tycolon> \<medium_left_bracket>\<medium_left_bracket> H\<^sub>m \<medium_right_bracket>\<medium_right_bracket> \<longmapsto> L \<heavy_asterisk> h\<^sub>m \<tycolon> H\<^sub>m \<medium_right_bracket>\<medium_right_bracket>"
+  unfolding Heap_Cast_Goal_def using cast_dual_id . *)
 
-lemma [\<nu>intro 1000]:
-  "\<medium_left_bracket>\<medium_left_bracket> \<^bold>c\<^bold>a\<^bold>s\<^bold>t h \<tycolon> H \<longmapsto> h \<tycolon> \<medium_left_bracket>\<medium_left_bracket> H \<medium_right_bracket>\<medium_right_bracket> \<medium_right_bracket>\<medium_right_bracket>"
-  unfolding Heap_Cast_Goal_def using cast_id .
+lemma heap_idx_this_dual[\<nu>intro 3000]:
+  "\<medium_left_bracket>\<medium_left_bracket> \<^bold>c\<^bold>a\<^bold>s\<^bold>t H \<longmapsto> \<medium_left_bracket>\<medium_left_bracket> H \<medium_right_bracket>\<medium_right_bracket> \<^bold>d\<^bold>u\<^bold>a\<^bold>l \<medium_left_bracket>\<medium_left_bracket> H\<^sub>m \<medium_right_bracket>\<medium_right_bracket> \<longmapsto> H\<^sub>m \<medium_right_bracket>\<medium_right_bracket>" unfolding Heap_Cast_Goal_def using cast_dual_id .
+lemma heap_idx_this_dual'[\<nu>intro 3000]:
+  "\<medium_left_bracket>\<medium_left_bracket> \<^bold>c\<^bold>a\<^bold>s\<^bold>t H \<longmapsto> Nothing \<heavy_asterisk> \<medium_left_bracket>\<medium_left_bracket> H \<medium_right_bracket>\<medium_right_bracket> \<^bold>d\<^bold>u\<^bold>a\<^bold>l Nothing \<heavy_asterisk> \<medium_left_bracket>\<medium_left_bracket> H\<^sub>m \<medium_right_bracket>\<medium_right_bracket> \<longmapsto> H\<^sub>m \<medium_right_bracket>\<medium_right_bracket>"
+  unfolding Heap_Cast_Goal_def Separation_emptyL Separation_emptyR using cast_dual_id .
 
-(* lemma [\<nu>intro 10]:
-  "\<^bold>c\<^bold>a\<^bold>s\<^bold>t h \<tycolon> H \<longmapsto> h' \<tycolon> H' \<^bold>w\<^bold>i\<^bold>t\<^bold>h P \<Longrightarrow>
-  \<medium_left_bracket>\<medium_left_bracket> \<^bold>c\<^bold>a\<^bold>s\<^bold>t h \<tycolon> H \<longmapsto> h' \<tycolon> \<medium_left_bracket>\<medium_left_bracket> H' \<medium_right_bracket>\<medium_right_bracket> \<^bold>w\<^bold>i\<^bold>t\<^bold>h P \<medium_right_bracket>\<medium_right_bracket>"
-  unfolding Heap_Cast_Goal_def  . *)
+lemma [\<nu>intro 3000]: "\<medium_left_bracket>\<medium_left_bracket> \<^bold>c\<^bold>a\<^bold>s\<^bold>t H \<longmapsto> \<medium_left_bracket>\<medium_left_bracket> H \<medium_right_bracket>\<medium_right_bracket> \<medium_right_bracket>\<medium_right_bracket>" and [\<nu>intro 3000]: "\<medium_left_bracket>\<medium_left_bracket> \<^bold>c\<^bold>a\<^bold>s\<^bold>t H \<longmapsto> Nothing \<heavy_asterisk> \<medium_left_bracket>\<medium_left_bracket> H \<medium_right_bracket>\<medium_right_bracket> \<medium_right_bracket>\<medium_right_bracket>"
+  unfolding Heap_Cast_Goal_def Separation_emptyL using cast_id by blast+
 
-lemma heap_idx_this_dual[\<nu>intro 1000]:
-  "\<medium_left_bracket>\<medium_left_bracket> \<^bold>c\<^bold>a\<^bold>s\<^bold>t x \<tycolon> X \<longmapsto> Nothing \<heavy_asterisk> x \<tycolon> \<medium_left_bracket>\<medium_left_bracket> X \<medium_right_bracket>\<medium_right_bracket> \<^bold>d\<^bold>u\<^bold>a\<^bold>l Nothing \<heavy_asterisk> x\<^sub>m \<tycolon> \<medium_left_bracket>\<medium_left_bracket> X\<^sub>m \<medium_right_bracket>\<medium_right_bracket> \<longmapsto> x\<^sub>m \<tycolon> X\<^sub>m \<medium_right_bracket>\<medium_right_bracket>"
+lemma [\<nu>intro 40]: \<comment> \<open>outro\<close>
+    "\<^bold>c\<^bold>a\<^bold>s\<^bold>t h \<tycolon> H \<longmapsto> H' \<heavy_asterisk> x \<tycolon> X \<^bold>w\<^bold>i\<^bold>t\<^bold>h P \<^bold>d\<^bold>u\<^bold>a\<^bold>l H'\<^sub>m \<heavy_asterisk> x\<^sub>m \<tycolon> X\<^sub>m \<longmapsto> h\<^sub>m \<tycolon> H\<^sub>m \<Longrightarrow>
+      \<medium_left_bracket>\<medium_left_bracket> \<^bold>c\<^bold>a\<^bold>s\<^bold>t h \<tycolon> H \<longmapsto> H' \<heavy_asterisk> \<medium_left_bracket>\<medium_left_bracket> x \<tycolon> X \<medium_right_bracket>\<medium_right_bracket> \<^bold>w\<^bold>i\<^bold>t\<^bold>h P \<^bold>d\<^bold>u\<^bold>a\<^bold>l H'\<^sub>m \<heavy_asterisk> \<medium_left_bracket>\<medium_left_bracket> x\<^sub>m \<tycolon> X\<^sub>m \<medium_right_bracket>\<medium_right_bracket> \<longmapsto> h\<^sub>m \<tycolon> H\<^sub>m \<medium_right_bracket>\<medium_right_bracket>"
+  and [\<nu>intro 40]:
+    "\<^bold>c\<^bold>a\<^bold>s\<^bold>t h \<tycolon> H \<longmapsto> H' \<heavy_asterisk> x \<tycolon> X \<^bold>w\<^bold>i\<^bold>t\<^bold>h P \<Longrightarrow> \<medium_left_bracket>\<medium_left_bracket> \<^bold>c\<^bold>a\<^bold>s\<^bold>t h \<tycolon> H \<longmapsto> H' \<heavy_asterisk> \<medium_left_bracket>\<medium_left_bracket> x \<tycolon> X \<medium_right_bracket>\<medium_right_bracket> \<^bold>w\<^bold>i\<^bold>t\<^bold>h P \<medium_right_bracket>\<medium_right_bracket>"
+  and [\<nu>intro 70]:
+    "\<^bold>c\<^bold>a\<^bold>s\<^bold>t h \<tycolon> H \<longmapsto> x \<tycolon> X \<^bold>w\<^bold>i\<^bold>t\<^bold>h P \<Longrightarrow> \<medium_left_bracket>\<medium_left_bracket> \<^bold>c\<^bold>a\<^bold>s\<^bold>t h \<tycolon> H \<longmapsto> Nothing \<heavy_asterisk> \<medium_left_bracket>\<medium_left_bracket> x \<tycolon> X \<medium_right_bracket>\<medium_right_bracket> \<^bold>w\<^bold>i\<^bold>t\<^bold>h P \<medium_right_bracket>\<medium_right_bracket>"
+  unfolding Heap_Cast_Goal_def Separation_emptyL .
+
+
+text \<open>to eliminate the Nothing hole that generated during the reasoning \<close>
+
+lemma heap_idx_dual_nothing[\<nu>intro 1200]:
+  "\<medium_left_bracket>\<medium_left_bracket> \<^bold>c\<^bold>a\<^bold>s\<^bold>t H \<longmapsto> \<medium_left_bracket>\<medium_left_bracket> X \<medium_right_bracket>\<medium_right_bracket> \<^bold>w\<^bold>i\<^bold>t\<^bold>h P \<^bold>d\<^bold>u\<^bold>a\<^bold>l H'\<^sub>m \<heavy_asterisk> \<medium_left_bracket>\<medium_left_bracket> X\<^sub>m \<medium_right_bracket>\<medium_right_bracket> \<longmapsto> H\<^sub>m \<medium_right_bracket>\<medium_right_bracket>
+  \<Longrightarrow> \<medium_left_bracket>\<medium_left_bracket> \<^bold>c\<^bold>a\<^bold>s\<^bold>t H \<heavy_asterisk> Nothing \<longmapsto> \<medium_left_bracket>\<medium_left_bracket> X \<medium_right_bracket>\<medium_right_bracket> \<^bold>w\<^bold>i\<^bold>t\<^bold>h P \<^bold>d\<^bold>u\<^bold>a\<^bold>l H'\<^sub>m \<heavy_asterisk> Nothing \<heavy_asterisk> \<medium_left_bracket>\<medium_left_bracket> X\<^sub>m \<medium_right_bracket>\<medium_right_bracket> \<longmapsto> H\<^sub>m \<heavy_asterisk> Nothing \<medium_right_bracket>\<medium_right_bracket>"
+  unfolding Cast_def CastDual_def Heap_Cast_Goal_def  Intro_def Dest_def Separation_emptyL Separation_emptyR .
+
+lemma [\<nu>intro 1200]:
+  "\<medium_left_bracket>\<medium_left_bracket> \<^bold>c\<^bold>a\<^bold>s\<^bold>t H \<longmapsto> \<medium_left_bracket>\<medium_left_bracket> X \<medium_right_bracket>\<medium_right_bracket> \<^bold>w\<^bold>i\<^bold>t\<^bold>h P \<medium_right_bracket>\<medium_right_bracket> \<Longrightarrow> \<medium_left_bracket>\<medium_left_bracket> \<^bold>c\<^bold>a\<^bold>s\<^bold>t H \<heavy_asterisk> Nothing \<longmapsto> \<medium_left_bracket>\<medium_left_bracket> X \<medium_right_bracket>\<medium_right_bracket> \<^bold>w\<^bold>i\<^bold>t\<^bold>h P \<medium_right_bracket>\<medium_right_bracket>"
+  unfolding Cast_def CastDual_def Heap_Cast_Goal_def  Intro_def Dest_def Separation_emptyL Separation_emptyR .
+
+lemma [\<nu>intro 1100]:
+  "\<medium_left_bracket>\<medium_left_bracket> \<^bold>c\<^bold>a\<^bold>s\<^bold>t H \<longmapsto> H1 \<heavy_asterisk> \<medium_left_bracket>\<medium_left_bracket> X \<medium_right_bracket>\<medium_right_bracket> \<^bold>w\<^bold>i\<^bold>t\<^bold>h P1 \<^bold>d\<^bold>u\<^bold>a\<^bold>l H1\<^sub>m \<heavy_asterisk> \<medium_left_bracket>\<medium_left_bracket> X\<^sub>m \<medium_right_bracket>\<medium_right_bracket> \<longmapsto> H\<^sub>m \<medium_right_bracket>\<medium_right_bracket>
+    \<Longrightarrow> (P1 \<Longrightarrow> \<medium_left_bracket>\<medium_left_bracket> \<^bold>c\<^bold>a\<^bold>s\<^bold>t H1 \<longmapsto> \<medium_left_bracket>\<medium_left_bracket> H2 \<medium_right_bracket>\<medium_right_bracket> \<^bold>w\<^bold>i\<^bold>t\<^bold>h P2 \<^bold>d\<^bold>u\<^bold>a\<^bold>l \<medium_left_bracket>\<medium_left_bracket> H2\<^sub>m \<medium_right_bracket>\<medium_right_bracket> \<longmapsto> H1\<^sub>m \<medium_right_bracket>\<medium_right_bracket>)
+    \<Longrightarrow> \<medium_left_bracket>\<medium_left_bracket> \<^bold>c\<^bold>a\<^bold>s\<^bold>t H \<longmapsto> \<medium_left_bracket>\<medium_left_bracket> H2 \<heavy_asterisk> X \<medium_right_bracket>\<medium_right_bracket> \<^bold>w\<^bold>i\<^bold>t\<^bold>h P1 \<and> P2 \<^bold>d\<^bold>u\<^bold>a\<^bold>l \<medium_left_bracket>\<medium_left_bracket> H2\<^sub>m \<heavy_asterisk> X\<^sub>m \<medium_right_bracket>\<medium_right_bracket> \<longmapsto> H\<^sub>m \<medium_right_bracket>\<medium_right_bracket>"
+  unfolding Cast_def CastDual_def Heap_Cast_Goal_def Intro_def Dest_def
+  by (metis Heap_Divider_exps)
+
+lemma [\<nu>intro 1100]:
+  "\<medium_left_bracket>\<medium_left_bracket> \<^bold>c\<^bold>a\<^bold>s\<^bold>t H \<longmapsto> H1 \<heavy_asterisk> \<medium_left_bracket>\<medium_left_bracket> X \<medium_right_bracket>\<medium_right_bracket> \<^bold>w\<^bold>i\<^bold>t\<^bold>h P \<medium_right_bracket>\<medium_right_bracket> \<Longrightarrow>
+  (P \<Longrightarrow> \<medium_left_bracket>\<medium_left_bracket> \<^bold>c\<^bold>a\<^bold>s\<^bold>t H1 \<longmapsto> \<medium_left_bracket>\<medium_left_bracket> H2 \<medium_right_bracket>\<medium_right_bracket> \<^bold>w\<^bold>i\<^bold>t\<^bold>h Q \<medium_right_bracket>\<medium_right_bracket>) \<Longrightarrow>
+  \<medium_left_bracket>\<medium_left_bracket> \<^bold>c\<^bold>a\<^bold>s\<^bold>t H \<longmapsto> \<medium_left_bracket>\<medium_left_bracket> H2 \<heavy_asterisk> X \<medium_right_bracket>\<medium_right_bracket> \<^bold>w\<^bold>i\<^bold>t\<^bold>h P \<and> Q \<medium_right_bracket>\<medium_right_bracket>"
+  unfolding Cast_def CastDual_def Heap_Cast_Goal_def Intro_def Dest_def
+  by (metis Heap_Divider_exps)
+
+(* lemma heap_idx_this_dual[\<nu>intro 1000]:
+  "\<medium_left_bracket>\<medium_left_bracket> \<^bold>c\<^bold>a\<^bold>s\<^bold>t x \<tycolon> X \<longmapsto> {Map.empty} \<heavy_asterisk> x \<tycolon> X \<^bold>d\<^bold>u\<^bold>a\<^bold>l {Map.empty} \<heavy_asterisk> x\<^sub>m \<tycolon> \<medium_left_bracket>\<medium_left_bracket> X\<^sub>m \<medium_right_bracket>\<medium_right_bracket> \<longmapsto> x\<^sub>m \<tycolon> X\<^sub>m \<medium_right_bracket>\<medium_right_bracket>"
   unfolding Cast_def Separation_emptyL Heap_Cast_Goal_def CastDual_def Intro_def Dest_def by simp
+*)
+
+  
 
 lemma heap_idx_L_dual[\<nu>intro 130]:
-  "\<medium_left_bracket>\<medium_left_bracket> \<^bold>c\<^bold>a\<^bold>s\<^bold>t h \<tycolon> H \<longmapsto> h' \<tycolon> H' \<heavy_asterisk> x \<tycolon> \<medium_left_bracket>\<medium_left_bracket> X \<medium_right_bracket>\<medium_right_bracket> \<^bold>w\<^bold>i\<^bold>t\<^bold>h P \<^bold>d\<^bold>u\<^bold>a\<^bold>l h'\<^sub>m \<tycolon> H'\<^sub>m \<heavy_asterisk> x\<^sub>m \<tycolon> \<medium_left_bracket>\<medium_left_bracket> X\<^sub>m \<medium_right_bracket>\<medium_right_bracket> \<longmapsto> h\<^sub>m \<tycolon> H\<^sub>m \<medium_right_bracket>\<medium_right_bracket>
-    \<Longrightarrow> \<medium_left_bracket>\<medium_left_bracket> \<^bold>c\<^bold>a\<^bold>s\<^bold>t l \<tycolon> L \<heavy_asterisk> h \<tycolon> H \<longmapsto> l \<tycolon> L \<heavy_asterisk> h' \<tycolon> H' \<heavy_asterisk> x \<tycolon> \<medium_left_bracket>\<medium_left_bracket> X \<medium_right_bracket>\<medium_right_bracket> \<^bold>w\<^bold>i\<^bold>t\<^bold>h P \<^bold>d\<^bold>u\<^bold>a\<^bold>l l \<tycolon> L \<heavy_asterisk> h'\<^sub>m \<tycolon> H'\<^sub>m \<heavy_asterisk> x\<^sub>m \<tycolon> \<medium_left_bracket>\<medium_left_bracket> X\<^sub>m \<medium_right_bracket>\<medium_right_bracket> \<longmapsto> l \<tycolon> L \<heavy_asterisk> h\<^sub>m \<tycolon> H\<^sub>m \<medium_right_bracket>\<medium_right_bracket>"
-  unfolding Cast_def CastDual_def Heap_Cast_Goal_def HeapDivNu_to_SepSet Intro_def Dest_def
-  by (smt (verit, del_insts) SeparationSet_assoc SeparationSet_comm SeparationSet_def mem_Collect_eq)
+  "\<medium_left_bracket>\<medium_left_bracket> \<^bold>c\<^bold>a\<^bold>s\<^bold>t H \<longmapsto> H' \<heavy_asterisk> \<medium_left_bracket>\<medium_left_bracket> x \<tycolon> X \<medium_right_bracket>\<medium_right_bracket> \<^bold>w\<^bold>i\<^bold>t\<^bold>h P \<^bold>d\<^bold>u\<^bold>a\<^bold>l H'\<^sub>m \<heavy_asterisk> \<medium_left_bracket>\<medium_left_bracket> x\<^sub>m \<tycolon> X\<^sub>m \<medium_right_bracket>\<medium_right_bracket> \<longmapsto> H\<^sub>m \<medium_right_bracket>\<medium_right_bracket>
+    \<Longrightarrow> \<medium_left_bracket>\<medium_left_bracket> \<^bold>c\<^bold>a\<^bold>s\<^bold>t L \<heavy_asterisk> H \<longmapsto> L \<heavy_asterisk> H' \<heavy_asterisk> \<medium_left_bracket>\<medium_left_bracket> x \<tycolon> X \<medium_right_bracket>\<medium_right_bracket> \<^bold>w\<^bold>i\<^bold>t\<^bold>h P \<^bold>d\<^bold>u\<^bold>a\<^bold>l L \<heavy_asterisk> H'\<^sub>m \<heavy_asterisk> \<medium_left_bracket>\<medium_left_bracket> x\<^sub>m \<tycolon> X\<^sub>m \<medium_right_bracket>\<medium_right_bracket> \<longmapsto> L \<heavy_asterisk> H\<^sub>m \<medium_right_bracket>\<medium_right_bracket>"
+  unfolding Cast_def CastDual_def Heap_Cast_Goal_def  Intro_def Dest_def
+  by (metis Heap_Divider_exps Separation_assoc)
 
-lemma heap_idx_L'[\<nu>intro 110]:
-  "\<medium_left_bracket>\<medium_left_bracket> \<^bold>c\<^bold>a\<^bold>s\<^bold>t h \<tycolon> H \<longmapsto> h' \<tycolon> H' \<heavy_asterisk> x \<tycolon> \<medium_left_bracket>\<medium_left_bracket> X \<medium_right_bracket>\<medium_right_bracket> \<^bold>w\<^bold>i\<^bold>t\<^bold>h P \<medium_right_bracket>\<medium_right_bracket>
-    \<Longrightarrow> \<medium_left_bracket>\<medium_left_bracket> \<^bold>c\<^bold>a\<^bold>s\<^bold>t l \<tycolon> L \<heavy_asterisk> h \<tycolon> H \<longmapsto> l \<tycolon> L \<heavy_asterisk> h' \<tycolon> H' \<heavy_asterisk> x \<tycolon> \<medium_left_bracket>\<medium_left_bracket> X \<medium_right_bracket>\<medium_right_bracket> \<^bold>w\<^bold>i\<^bold>t\<^bold>h P \<medium_right_bracket>\<medium_right_bracket>"
-  unfolding Cast_def CastDual_def Heap_Cast_Goal_def HeapDivNu_to_SepSet Intro_def Dest_def
-  by (smt (verit, del_insts) SeparationSet_assoc SeparationSet_comm SeparationSet_def mem_Collect_eq)
+lemma heap_idx_L[\<nu>intro 110]:
+  "\<medium_left_bracket>\<medium_left_bracket> \<^bold>c\<^bold>a\<^bold>s\<^bold>t H \<longmapsto> H' \<heavy_asterisk> \<medium_left_bracket>\<medium_left_bracket> x \<tycolon> X \<medium_right_bracket>\<medium_right_bracket> \<^bold>w\<^bold>i\<^bold>t\<^bold>h P \<medium_right_bracket>\<medium_right_bracket> \<Longrightarrow> \<medium_left_bracket>\<medium_left_bracket> \<^bold>c\<^bold>a\<^bold>s\<^bold>t L \<heavy_asterisk> H \<longmapsto> L \<heavy_asterisk> H' \<heavy_asterisk> \<medium_left_bracket>\<medium_left_bracket> x \<tycolon> X \<medium_right_bracket>\<medium_right_bracket> \<^bold>w\<^bold>i\<^bold>t\<^bold>h P \<medium_right_bracket>\<medium_right_bracket>"
+  unfolding Cast_def CastDual_def Heap_Cast_Goal_def Intro_def Dest_def
+  by (metis Heap_Divider_exps Separation_assoc)
 
-lemma heap_idx_L[\<nu>intro 130]:
-  "\<^bold>c\<^bold>a\<^bold>s\<^bold>t h \<tycolon> H \<longmapsto> x \<tycolon> X \<^bold>w\<^bold>i\<^bold>t\<^bold>h P \<Longrightarrow> \<medium_left_bracket>\<medium_left_bracket> \<^bold>c\<^bold>a\<^bold>s\<^bold>t l \<tycolon> L \<heavy_asterisk> h \<tycolon> H \<longmapsto> l \<tycolon> L \<heavy_asterisk> x \<tycolon> \<medium_left_bracket>\<medium_left_bracket> X \<medium_right_bracket>\<medium_right_bracket> \<^bold>w\<^bold>i\<^bold>t\<^bold>h P \<medium_right_bracket>\<medium_right_bracket>"
-  unfolding Cast_def CastDual_def Heap_Cast_Goal_def HeapDivNu_to_SepSet Intro_def Dest_def
-  by (smt (verit, del_insts) SeparationSet_assoc SeparationSet_comm SeparationSet_def mem_Collect_eq)
 
-lemma heap_idx_R_dual[\<nu>intro]:
-  "\<medium_left_bracket>\<medium_left_bracket> \<^bold>c\<^bold>a\<^bold>s\<^bold>t h \<tycolon> H \<longmapsto> h' \<tycolon> H' \<heavy_asterisk> x \<tycolon> \<medium_left_bracket>\<medium_left_bracket> X \<medium_right_bracket>\<medium_right_bracket> \<^bold>w\<^bold>i\<^bold>t\<^bold>h P
-      \<^bold>d\<^bold>u\<^bold>a\<^bold>l h'\<^sub>m \<tycolon> H'\<^sub>m \<heavy_asterisk> x\<^sub>m \<tycolon> \<medium_left_bracket>\<medium_left_bracket> X\<^sub>m \<medium_right_bracket>\<medium_right_bracket> \<longmapsto> h\<^sub>m \<tycolon> H\<^sub>m \<medium_right_bracket>\<medium_right_bracket>
-  \<Longrightarrow> \<medium_left_bracket>\<medium_left_bracket> \<^bold>c\<^bold>a\<^bold>s\<^bold>t h \<tycolon> H \<heavy_asterisk> r \<tycolon> R \<longmapsto> h' \<tycolon> H' \<heavy_asterisk> r \<tycolon> R \<heavy_asterisk> x \<tycolon> \<medium_left_bracket>\<medium_left_bracket> X \<medium_right_bracket>\<medium_right_bracket> \<^bold>w\<^bold>i\<^bold>t\<^bold>h P
-      \<^bold>d\<^bold>u\<^bold>a\<^bold>l h'\<^sub>m \<tycolon> H'\<^sub>m \<heavy_asterisk> r \<tycolon> R \<heavy_asterisk> x\<^sub>m \<tycolon> \<medium_left_bracket>\<medium_left_bracket> X\<^sub>m \<medium_right_bracket>\<medium_right_bracket> \<longmapsto> h\<^sub>m \<tycolon> H\<^sub>m \<heavy_asterisk> r \<tycolon> R \<medium_right_bracket>\<medium_right_bracket>"
-  unfolding Cast_def CastDual_def Heap_Cast_Goal_def HeapDivNu_to_SepSet Intro_def Dest_def
-  by (smt (verit, del_insts) SeparationSet_assoc SeparationSet_comm SeparationSet_def mem_Collect_eq)
+lemma heap_idx_R_dual[\<nu>intro 100]:
+  "\<medium_left_bracket>\<medium_left_bracket> \<^bold>c\<^bold>a\<^bold>s\<^bold>t H \<longmapsto> H' \<heavy_asterisk> \<medium_left_bracket>\<medium_left_bracket> x \<tycolon> X \<medium_right_bracket>\<medium_right_bracket> \<^bold>w\<^bold>i\<^bold>t\<^bold>h P \<^bold>d\<^bold>u\<^bold>a\<^bold>l H'\<^sub>m \<heavy_asterisk> \<medium_left_bracket>\<medium_left_bracket> x\<^sub>m \<tycolon> X\<^sub>m \<medium_right_bracket>\<medium_right_bracket> \<longmapsto> H\<^sub>m \<medium_right_bracket>\<medium_right_bracket>
+  \<Longrightarrow> \<medium_left_bracket>\<medium_left_bracket> \<^bold>c\<^bold>a\<^bold>s\<^bold>t H \<heavy_asterisk> R \<longmapsto> H' \<heavy_asterisk> R \<heavy_asterisk> \<medium_left_bracket>\<medium_left_bracket> x \<tycolon> X \<medium_right_bracket>\<medium_right_bracket> \<^bold>w\<^bold>i\<^bold>t\<^bold>h P \<^bold>d\<^bold>u\<^bold>a\<^bold>l H'\<^sub>m \<heavy_asterisk> R \<heavy_asterisk> \<medium_left_bracket>\<medium_left_bracket> x\<^sub>m \<tycolon> X\<^sub>m \<medium_right_bracket>\<medium_right_bracket> \<longmapsto> H\<^sub>m \<heavy_asterisk> R \<medium_right_bracket>\<medium_right_bracket>"
+  unfolding Cast_def CastDual_def Heap_Cast_Goal_def Intro_def Dest_def
+    Separation_comm[of H R] Separation_comm[of H\<^sub>m R]
+    Separation_comm[of H' R] Separation_comm[of H'\<^sub>m R]
+  by (metis Heap_Divider_exps Separation_assoc)
 
-lemma heap_idx_R[\<nu>intro]:
-  "\<medium_left_bracket>\<medium_left_bracket> \<^bold>c\<^bold>a\<^bold>s\<^bold>t h \<tycolon> H \<longmapsto> h' \<tycolon> H' \<heavy_asterisk> x \<tycolon> \<medium_left_bracket>\<medium_left_bracket> X \<medium_right_bracket>\<medium_right_bracket> \<^bold>w\<^bold>i\<^bold>t\<^bold>h P \<medium_right_bracket>\<medium_right_bracket>
-    \<Longrightarrow> \<medium_left_bracket>\<medium_left_bracket> \<^bold>c\<^bold>a\<^bold>s\<^bold>t h \<tycolon> H \<heavy_asterisk> r \<tycolon> R \<longmapsto> h' \<tycolon> H' \<heavy_asterisk> r \<tycolon> R \<heavy_asterisk> x \<tycolon> \<medium_left_bracket>\<medium_left_bracket> X \<medium_right_bracket>\<medium_right_bracket> \<^bold>w\<^bold>i\<^bold>t\<^bold>h P \<medium_right_bracket>\<medium_right_bracket>"
-  unfolding Cast_def CastDual_def Heap_Cast_Goal_def HeapDivNu_to_SepSet Intro_def Dest_def
-  by (smt (verit, del_insts) SeparationSet_assoc SeparationSet_comm SeparationSet_def mem_Collect_eq)
+lemma heap_idx_R[\<nu>intro 100]:
+  "\<medium_left_bracket>\<medium_left_bracket> \<^bold>c\<^bold>a\<^bold>s\<^bold>t H \<longmapsto> H' \<heavy_asterisk> \<medium_left_bracket>\<medium_left_bracket> x \<tycolon> X \<medium_right_bracket>\<medium_right_bracket> \<^bold>w\<^bold>i\<^bold>t\<^bold>h P \<medium_right_bracket>\<medium_right_bracket> \<Longrightarrow> \<medium_left_bracket>\<medium_left_bracket> \<^bold>c\<^bold>a\<^bold>s\<^bold>t H \<heavy_asterisk> R \<longmapsto> H' \<heavy_asterisk> R \<heavy_asterisk> \<medium_left_bracket>\<medium_left_bracket> x \<tycolon> X \<medium_right_bracket>\<medium_right_bracket> \<^bold>w\<^bold>i\<^bold>t\<^bold>h P \<medium_right_bracket>\<medium_right_bracket>"
+  unfolding Cast_def CastDual_def Heap_Cast_Goal_def Intro_def Dest_def
+    Separation_comm[of H R] Separation_comm[of H' R]
+  by (metis Heap_Divider_exps Separation_assoc)
 
-lemma [\<nu>intro 200]:
-  "\<medium_left_bracket>\<medium_left_bracket> \<^bold>c\<^bold>a\<^bold>s\<^bold>t h \<tycolon> H \<longmapsto> h1 \<tycolon> H1 \<heavy_asterisk> x \<tycolon> \<medium_left_bracket>\<medium_left_bracket> X \<medium_right_bracket>\<medium_right_bracket> \<^bold>w\<^bold>i\<^bold>t\<^bold>h P1 \<^bold>d\<^bold>u\<^bold>a\<^bold>l h1\<^sub>m \<tycolon> H1\<^sub>m \<heavy_asterisk> x\<^sub>m \<tycolon> \<medium_left_bracket>\<medium_left_bracket> X\<^sub>m \<medium_right_bracket>\<medium_right_bracket> \<longmapsto> h\<^sub>m \<tycolon> H\<^sub>m  \<medium_right_bracket>\<medium_right_bracket>
-    \<Longrightarrow> (P1 \<Longrightarrow> \<medium_left_bracket>\<medium_left_bracket> \<^bold>c\<^bold>a\<^bold>s\<^bold>t h1 \<tycolon> H1 \<longmapsto> h2 \<tycolon> \<medium_left_bracket>\<medium_left_bracket> H2 \<medium_right_bracket>\<medium_right_bracket> \<^bold>w\<^bold>i\<^bold>t\<^bold>h P2 \<^bold>d\<^bold>u\<^bold>a\<^bold>l h2\<^sub>m \<tycolon> \<medium_left_bracket>\<medium_left_bracket> H2\<^sub>m \<medium_right_bracket>\<medium_right_bracket> \<longmapsto> h1\<^sub>m \<tycolon> H1\<^sub>m \<medium_right_bracket>\<medium_right_bracket>)
-    \<Longrightarrow> \<medium_left_bracket>\<medium_left_bracket> \<^bold>c\<^bold>a\<^bold>s\<^bold>t h \<tycolon> H \<longmapsto> (x, h2) \<tycolon> \<medium_left_bracket>\<medium_left_bracket> X <heap-sep> H2 \<medium_right_bracket>\<medium_right_bracket> \<^bold>w\<^bold>i\<^bold>t\<^bold>h P1 \<and> P2 \<^bold>d\<^bold>u\<^bold>a\<^bold>l (x\<^sub>m, h2\<^sub>m) \<tycolon> \<medium_left_bracket>\<medium_left_bracket> X\<^sub>m <heap-sep> H2\<^sub>m \<medium_right_bracket>\<medium_right_bracket> \<longmapsto> h\<^sub>m \<tycolon> H\<^sub>m \<medium_right_bracket>\<medium_right_bracket>"
-  unfolding Cast_def CastDual_def Heap_Cast_Goal_def HeapDivNu_to_SepSet Intro_def Dest_def
-  by (smt (verit, del_insts) SeparationSet_assoc SeparationSet_comm SeparationSet_def mem_Collect_eq)
-
-lemma [\<nu>intro 200]:
-  "\<medium_left_bracket>\<medium_left_bracket> \<^bold>c\<^bold>a\<^bold>s\<^bold>t h \<tycolon> H \<longmapsto> h1 \<tycolon> H1 \<heavy_asterisk> x \<tycolon> \<medium_left_bracket>\<medium_left_bracket> X \<medium_right_bracket>\<medium_right_bracket> \<^bold>w\<^bold>i\<^bold>t\<^bold>h P1 \<medium_right_bracket>\<medium_right_bracket>
-    \<Longrightarrow> (P1 \<Longrightarrow> \<medium_left_bracket>\<medium_left_bracket> \<^bold>c\<^bold>a\<^bold>s\<^bold>t h1 \<tycolon> H1 \<longmapsto> h2 \<tycolon> \<medium_left_bracket>\<medium_left_bracket> H2 \<medium_right_bracket>\<medium_right_bracket> \<^bold>w\<^bold>i\<^bold>t\<^bold>h P2 \<medium_right_bracket>\<medium_right_bracket>)
-    \<Longrightarrow> \<medium_left_bracket>\<medium_left_bracket> \<^bold>c\<^bold>a\<^bold>s\<^bold>t h \<tycolon> H \<longmapsto> (x, h2) \<tycolon> \<medium_left_bracket>\<medium_left_bracket> X <heap-sep> H2 \<medium_right_bracket>\<medium_right_bracket> \<^bold>w\<^bold>i\<^bold>t\<^bold>h P1 \<and> P2 \<medium_right_bracket>\<medium_right_bracket>"
-  unfolding Cast_def CastDual_def Heap_Cast_Goal_def HeapDivNu_to_SepSet Intro_def Dest_def
-  by (smt (verit, del_insts) SeparationSet_assoc SeparationSet_comm SeparationSet_def mem_Collect_eq)
 
 lemma [\<nu>intro 120]:
-  "\<medium_left_bracket>\<medium_left_bracket> \<^bold>c\<^bold>a\<^bold>s\<^bold>t h \<tycolon> H \<longmapsto> h1 \<tycolon> H1 \<heavy_asterisk> x \<tycolon> \<medium_left_bracket>\<medium_left_bracket> X \<medium_right_bracket>\<medium_right_bracket> \<^bold>w\<^bold>i\<^bold>t\<^bold>h P1 \<medium_right_bracket>\<medium_right_bracket>
+  "\<medium_left_bracket>\<medium_left_bracket> \<^bold>c\<^bold>a\<^bold>s\<^bold>t H \<longmapsto> H1 \<heavy_asterisk> x \<tycolon> \<medium_left_bracket>\<medium_left_bracket> X \<medium_right_bracket>\<medium_right_bracket> \<^bold>w\<^bold>i\<^bold>t\<^bold>h P1 \<medium_right_bracket>\<medium_right_bracket>
     \<Longrightarrow> (P1 \<Longrightarrow> \<medium_left_bracket>\<medium_left_bracket> \<^bold>c\<^bold>a\<^bold>s\<^bold>t h1 \<tycolon> H1 \<longmapsto> h\<^sub>r \<tycolon> H\<^sub>r \<heavy_asterisk> h2 \<tycolon> \<medium_left_bracket>\<medium_left_bracket> H2 \<medium_right_bracket>\<medium_right_bracket> \<^bold>w\<^bold>i\<^bold>t\<^bold>h P2 \<medium_right_bracket>\<medium_right_bracket>)
     \<Longrightarrow> \<medium_left_bracket>\<medium_left_bracket> \<^bold>c\<^bold>a\<^bold>s\<^bold>t h \<tycolon> H \<longmapsto> h\<^sub>r \<tycolon> H\<^sub>r \<heavy_asterisk> (x, h2) \<tycolon> \<medium_left_bracket>\<medium_left_bracket> X \<^emph> H2 \<medium_right_bracket>\<medium_right_bracket> \<^bold>w\<^bold>i\<^bold>t\<^bold>h P1 \<and> P2 \<medium_right_bracket>\<medium_right_bracket>"
   unfolding Cast_def CastDual_def Heap_Cast_Goal_def HeapDivNu_to_SepSet SepNu_to_SepSet Intro_def Dest_def
   by (smt (verit, del_insts) SeparationSet_assoc SeparationSet_comm SeparationSet_def mem_Collect_eq)
 
-lemma [ \<nu>intro -50 ]: "\<^bold>d\<^bold>e\<^bold>s\<^bold>t \<^bold>c\<^bold>a\<^bold>s\<^bold>t x \<tycolon> T \<longmapsto> d \<tycolon> D \<^bold>w\<^bold>i\<^bold>t\<^bold>h P
+(* lemma [ \<nu>intro -50 ]: "\<^bold>d\<^bold>e\<^bold>s\<^bold>t \<^bold>c\<^bold>a\<^bold>s\<^bold>t x \<tycolon> T \<longmapsto> d \<tycolon> D \<^bold>w\<^bold>i\<^bold>t\<^bold>h P
   \<Longrightarrow> (P \<Longrightarrow> \<medium_left_bracket>\<medium_left_bracket> \<^bold>c\<^bold>a\<^bold>s\<^bold>t d \<tycolon> D \<longmapsto> d' \<tycolon> D' \<heavy_asterisk> h \<tycolon> \<medium_left_bracket>\<medium_left_bracket> H \<medium_right_bracket>\<medium_right_bracket> \<^bold>w\<^bold>i\<^bold>t\<^bold>h P2 \<^bold>d\<^bold>u\<^bold>a\<^bold>l i'\<^sub>m \<tycolon> I'\<^sub>m \<heavy_asterisk> h\<^sub>m \<tycolon> \<medium_left_bracket>\<medium_left_bracket> H\<^sub>m \<medium_right_bracket>\<medium_right_bracket> \<longmapsto> i \<tycolon> I \<medium_right_bracket>\<medium_right_bracket>)
   \<Longrightarrow> (P \<Longrightarrow> P2 \<Longrightarrow> \<^bold>i\<^bold>n\<^bold>t\<^bold>r\<^bold>o \<^bold>c\<^bold>a\<^bold>s\<^bold>t i \<tycolon> I \<longmapsto> x\<^sub>m \<tycolon> T \<^bold>w\<^bold>i\<^bold>t\<^bold>h Anyway)
   \<Longrightarrow> \<medium_left_bracket>\<medium_left_bracket> \<^bold>c\<^bold>a\<^bold>s\<^bold>t x \<tycolon> T \<longmapsto> d' \<tycolon> D' \<heavy_asterisk> h \<tycolon> \<medium_left_bracket>\<medium_left_bracket> H \<medium_right_bracket>\<medium_right_bracket> \<^bold>w\<^bold>i\<^bold>t\<^bold>h P \<and> P2 \<^bold>d\<^bold>u\<^bold>a\<^bold>l i'\<^sub>m \<tycolon> I'\<^sub>m \<heavy_asterisk> h\<^sub>m \<tycolon> \<medium_left_bracket>\<medium_left_bracket> H\<^sub>m \<medium_right_bracket>\<medium_right_bracket> \<longmapsto> x\<^sub>m \<tycolon> T \<medium_right_bracket>\<medium_right_bracket>"
   unfolding Dest_def Intro_def CastDual_def Different_def Heap_Cast_Goal_def Cast_def
-  by (auto simp add: Premise_def)
+  by (auto simp add: Premise_def) *)
 
 (* lemma [ \<nu>intro 50 ]: "\<^bold>c\<^bold>a\<^bold>s\<^bold>t x \<tycolon> T \<longmapsto> d \<tycolon> D \<^bold>w\<^bold>i\<^bold>t\<^bold>h P
   \<Longrightarrow> (P \<Longrightarrow> \<medium_left_bracket>\<medium_left_bracket> \<^bold>c\<^bold>a\<^bold>s\<^bold>t d \<tycolon> D \<longmapsto> d' \<tycolon> D' \<heavy_asterisk> h \<tycolon> \<medium_left_bracket>\<medium_left_bracket> H \<medium_right_bracket>\<medium_right_bracket> \<^bold>w\<^bold>i\<^bold>t\<^bold>h P2 \<^bold>d\<^bold>u\<^bold>a\<^bold>l i'\<^sub>m \<tycolon> I'\<^sub>m \<heavy_asterisk> h\<^sub>m \<tycolon> \<medium_left_bracket>\<medium_left_bracket> H\<^sub>m \<medium_right_bracket>\<medium_right_bracket> \<longmapsto> i \<tycolon> I \<medium_right_bracket>\<medium_right_bracket>)
@@ -1076,9 +1113,6 @@ lemma StackDelimiter_to_AndTy: " (A\<heavy_comma> B) \<equiv> (B \<^bold>a\<^bol
 
 subsection \<open>Cast\<close>
 
-
-lemma apply_cast: "(\<^bold>c\<^bold>u\<^bold>r\<^bold>r\<^bold>e\<^bold>n\<^bold>t blk \<^bold>r\<^bold>e\<^bold>s\<^bold>u\<^bold>l\<^bold>t\<^bold>s \<^bold>i\<^bold>n (R \<heavy_comma> x \<tycolon> X\<heavy_comma> \<^bold>h\<^bold>e\<^bold>a\<^bold>p H)) \<Longrightarrow> (\<^bold>c\<^bold>a\<^bold>s\<^bold>t x \<tycolon> X \<longmapsto> y \<tycolon> Y \<^bold>w\<^bold>i\<^bold>t\<^bold>h P) \<Longrightarrow> (\<^bold>c\<^bold>u\<^bold>r\<^bold>r\<^bold>e\<^bold>n\<^bold>t blk \<^bold>r\<^bold>e\<^bold>s\<^bold>u\<^bold>l\<^bold>t\<^bold>s \<^bold>i\<^bold>n (R \<heavy_comma> y \<tycolon> Y\<heavy_comma> \<^bold>h\<^bold>e\<^bold>a\<^bold>p H) \<and> P)"
-  unfolding Procedure_def CurrentConstruction_def PendingConstruction_def bind_def SpecTop_imp Cast_def by (auto 4 6 simp add: nu_exps)
 lemma "cast": "\<^bold>c\<^bold>u\<^bold>r\<^bold>r\<^bold>e\<^bold>n\<^bold>t blk \<^bold>r\<^bold>e\<^bold>s\<^bold>u\<^bold>l\<^bold>t\<^bold>s \<^bold>i\<^bold>n T \<Longrightarrow> \<^bold>c\<^bold>a\<^bold>s\<^bold>t T \<longmapsto> T' \<^bold>w\<^bold>i\<^bold>t\<^bold>h P \<Longrightarrow> \<^bold>c\<^bold>u\<^bold>r\<^bold>r\<^bold>e\<^bold>n\<^bold>t blk \<^bold>r\<^bold>e\<^bold>s\<^bold>u\<^bold>l\<^bold>t\<^bold>s \<^bold>i\<^bold>n T' "
   for T' :: "(heap \<times> 'a::lrep) set" unfolding Cast_def CurrentConstruction_def by auto
 lemma "cast'": "\<^bold>p\<^bold>e\<^bold>n\<^bold>d\<^bold>i\<^bold>n\<^bold>g f \<^bold>o\<^bold>n blk \<^bold>r\<^bold>e\<^bold>s\<^bold>u\<^bold>l\<^bold>t\<^bold>s \<^bold>i\<^bold>n T \<Longrightarrow> \<^bold>c\<^bold>a\<^bold>s\<^bold>t T \<longmapsto> T' \<^bold>w\<^bold>i\<^bold>t\<^bold>h P \<Longrightarrow> \<^bold>p\<^bold>e\<^bold>n\<^bold>d\<^bold>i\<^bold>n\<^bold>g f \<^bold>o\<^bold>n blk \<^bold>r\<^bold>e\<^bold>s\<^bold>u\<^bold>l\<^bold>t\<^bold>s \<^bold>i\<^bold>n T' "
@@ -1088,18 +1122,18 @@ lemma cast_\<nu>app: "\<^bold>a\<^bold>r\<^bold>g\<^bold>u\<^bold>m\<^bold>e\<^b
   unfolding Cast_def Argument_def by (simp add: nu_exps) blast
 
 lemma cast_heap_\<nu>app:
-  "\<^bold>a\<^bold>r\<^bold>g\<^bold>u\<^bold>m\<^bold>e\<^bold>n\<^bold>t \<^bold>c\<^bold>a\<^bold>s\<^bold>t x \<tycolon> X \<longmapsto> x' \<tycolon> X' \<^bold>w\<^bold>i\<^bold>t\<^bold>h P \<Longrightarrow> \<^bold>c\<^bold>a\<^bold>s\<^bold>t R\<heavy_comma> \<^bold>h\<^bold>e\<^bold>a\<^bold>p H \<heavy_asterisk> x \<tycolon> X \<longmapsto> R\<heavy_comma> \<^bold>h\<^bold>e\<^bold>a\<^bold>p H \<heavy_asterisk> x' \<tycolon> X' \<^bold>w\<^bold>i\<^bold>t\<^bold>h P"
-  unfolding Cast_def Argument_def Heap_Delimiter_def by (simp add: nu_exps) blast
+  "\<^bold>a\<^bold>r\<^bold>g\<^bold>u\<^bold>m\<^bold>e\<^bold>n\<^bold>t \<^bold>c\<^bold>a\<^bold>s\<^bold>t X \<longmapsto> X' \<^bold>w\<^bold>i\<^bold>t\<^bold>h P \<Longrightarrow> \<^bold>c\<^bold>a\<^bold>s\<^bold>t R\<heavy_comma> \<^bold>h\<^bold>e\<^bold>a\<^bold>p H \<heavy_asterisk> X \<longmapsto> R\<heavy_comma> \<^bold>h\<^bold>e\<^bold>a\<^bold>p H \<heavy_asterisk> X' \<^bold>w\<^bold>i\<^bold>t\<^bold>h P"
+  unfolding Cast_def Argument_def Heap_Divider_def by (simp add: nu_exps) blast
 
 lemma cast_whole_heap_\<nu>app:
-  "\<^bold>a\<^bold>r\<^bold>g\<^bold>u\<^bold>m\<^bold>e\<^bold>n\<^bold>t \<^bold>c\<^bold>a\<^bold>s\<^bold>t h \<tycolon> H \<longmapsto> h' \<tycolon> H' \<^bold>w\<^bold>i\<^bold>t\<^bold>h P \<Longrightarrow> \<^bold>c\<^bold>a\<^bold>s\<^bold>t R\<heavy_comma> \<^bold>h\<^bold>e\<^bold>a\<^bold>p h \<tycolon> H \<longmapsto> R\<heavy_comma> \<^bold>h\<^bold>e\<^bold>a\<^bold>p h' \<tycolon> H' \<^bold>w\<^bold>i\<^bold>t\<^bold>h P"
+  "\<^bold>a\<^bold>r\<^bold>g\<^bold>u\<^bold>m\<^bold>e\<^bold>n\<^bold>t \<^bold>c\<^bold>a\<^bold>s\<^bold>t H \<longmapsto> H' \<^bold>w\<^bold>i\<^bold>t\<^bold>h P \<Longrightarrow> \<^bold>c\<^bold>a\<^bold>s\<^bold>t R\<heavy_comma> \<^bold>h\<^bold>e\<^bold>a\<^bold>p H \<longmapsto> R\<heavy_comma> \<^bold>h\<^bold>e\<^bold>a\<^bold>p H' \<^bold>w\<^bold>i\<^bold>t\<^bold>h P"
   unfolding Cast_def Argument_def by (simp add: nu_exps) blast
 
 lemma cast_heap_conversion:
-  "\<medium_left_bracket>\<medium_left_bracket> \<^bold>c\<^bold>a\<^bold>s\<^bold>t h\<^sub>x \<tycolon> H\<^sub>x \<longmapsto> h\<^sub>r \<tycolon> H\<^sub>r \<heavy_asterisk> h \<tycolon> \<medium_left_bracket>\<medium_left_bracket> H \<medium_right_bracket>\<medium_right_bracket> \<^bold>w\<^bold>i\<^bold>t\<^bold>h Any \<medium_right_bracket>\<medium_right_bracket>
+  "\<medium_left_bracket>\<medium_left_bracket> \<^bold>c\<^bold>a\<^bold>s\<^bold>t H\<^sub>x \<longmapsto> H\<^sub>r \<heavy_asterisk> h \<tycolon> H \<^bold>w\<^bold>i\<^bold>t\<^bold>h Any \<medium_right_bracket>\<medium_right_bracket>
   \<Longrightarrow> \<^bold>c\<^bold>a\<^bold>s\<^bold>t h \<tycolon> H \<longmapsto> h' \<tycolon> H' \<^bold>w\<^bold>i\<^bold>t\<^bold>h P
-  \<Longrightarrow> \<^bold>c\<^bold>a\<^bold>s\<^bold>t h\<^sub>x \<tycolon> H\<^sub>x \<longmapsto> h\<^sub>r \<tycolon> H\<^sub>r \<heavy_asterisk> h' \<tycolon> H' \<^bold>w\<^bold>i\<^bold>t\<^bold>h P"
-  unfolding Cast_def Heap_Cast_Goal_def Heap_Delimiter_def by (simp add: nu_exps) blast
+  \<Longrightarrow> \<^bold>c\<^bold>a\<^bold>s\<^bold>t H\<^sub>x \<longmapsto> H\<^sub>r \<heavy_asterisk> h' \<tycolon> H' \<^bold>w\<^bold>i\<^bold>t\<^bold>h P"
+  unfolding Cast_def Heap_Cast_Goal_def Heap_Divider_def by (simp add: nu_exps) blast
 
 (* theorem proc_cast': "\<^bold>p\<^bold>r\<^bold>o\<^bold>c f \<blangle> A \<longmapsto> B \<brangle> \<Longrightarrow> \<^bold>c\<^bold>a\<^bold>s\<^bold>t A' \<longmapsto> A \<^bold>w\<^bold>i\<^bold>t\<^bold>h P \<Longrightarrow> \<^bold>c\<^bold>a\<^bold>s\<^bold>t B \<longmapsto> B' \<^bold>w\<^bold>i\<^bold>t\<^bold>h Q \<Longrightarrow> \<^bold>p\<^bold>r\<^bold>o\<^bold>c f \<blangle> A' \<longmapsto> B' \<brangle>"
   unfolding Procedure_def Cast_def by (auto 0 4) *)
@@ -1149,13 +1183,17 @@ definition Arguments :: " (heap \<times> 'a) set \<Rightarrow> (heap \<times> 'b
   "Arguments A B R args \<longleftrightarrow> (\<forall>h a. (h,a) \<in> A \<longrightarrow> (h, fst (assemble_arg args a)) \<in> B \<and> snd (assemble_arg args a) \<in> R)
     \<and> (\<forall>h b r. (h,b) \<in> B \<and> r \<in> R \<longrightarrow> (h, dissemble_arg args (b,r)) \<in> A)"
 
-lemma [\<nu>intro]: "Arguments \<tort_lbrace>r \<tycolon> R\<heavy_comma> \<^bold>h\<^bold>e\<^bold>a\<^bold>p H\<tort_rbrace> \<tort_lbrace>Void\<heavy_comma> \<^bold>h\<^bold>e\<^bold>a\<^bold>p H\<tort_rbrace> \<tort_lbrace>r \<tycolon> R\<tort_rbrace> no_argument"
+lemma [\<nu>intro]: "Arguments (R\<heavy_comma> \<^bold>h\<^bold>e\<^bold>a\<^bold>p H) (Void\<heavy_comma> \<^bold>h\<^bold>e\<^bold>a\<^bold>p H) R no_argument"
   unfolding no_argument_def Arguments_def by (simp add: nu_exps)
-lemma [\<nu>intro]: "Arguments \<tort_lbrace>a \<tycolon> A\<heavy_comma> \<^bold>h\<^bold>e\<^bold>a\<^bold>p H\<tort_rbrace> \<tort_lbrace>b \<tycolon> B\<heavy_comma> \<^bold>h\<^bold>e\<^bold>a\<^bold>p H\<tort_rbrace> R args
-  \<Longrightarrow> Arguments \<tort_lbrace>a \<tycolon> A\<heavy_comma> x \<tycolon> X\<heavy_comma> \<^bold>h\<^bold>e\<^bold>a\<^bold>p H\<tort_rbrace> \<tort_lbrace>b \<tycolon> B\<heavy_comma> x \<tycolon> X\<heavy_comma> \<^bold>h\<^bold>e\<^bold>a\<^bold>p H\<tort_rbrace> R (and_argument args TYPE('xp))"
-  for X :: "('xp::lrep, 'x) \<nu>" unfolding and_argument_def Arguments_def by (cases args) (auto 0 3 split: prod.split simp add: nu_exps) 
-lemma [\<nu>intro]: "(\<And>c. Arguments \<tort_lbrace>x c \<tycolon> T c\<tort_rbrace> \<tort_lbrace>x' c \<tycolon> T' c\<tort_rbrace> R arg) \<Longrightarrow> Arguments \<tort_lbrace>x \<tycolon> ExNu T\<tort_rbrace> \<tort_lbrace>x' \<tycolon> ExNu T'\<tort_rbrace> R arg"
+
+lemma [\<nu>intro]: "Arguments (A\<heavy_comma> \<^bold>h\<^bold>e\<^bold>a\<^bold>p H) (B\<heavy_comma> \<^bold>h\<^bold>e\<^bold>a\<^bold>p H) R args
+  \<Longrightarrow> Arguments (A\<heavy_comma> x \<tycolon> X\<heavy_comma> \<^bold>h\<^bold>e\<^bold>a\<^bold>p H) (B\<heavy_comma> x \<tycolon> X\<heavy_comma> \<^bold>h\<^bold>e\<^bold>a\<^bold>p H) R (and_argument args TYPE('xp))"
+  for X :: "('xp::lrep, 'x) \<nu>" unfolding and_argument_def Arguments_def
+  by (cases args) (auto 0 3 split: prod.split simp add: nu_exps) 
+
+lemma [\<nu>intro]: "(\<And>c. Arguments (T c) (T' c) R arg) \<Longrightarrow> Arguments (ExSet T) (ExSet T') R arg"
   unfolding Arguments_def by (simp add: nu_exps) blast
+
 
 definition op_call :: " ('r1, 'a \<times> 'r2) argument_types \<Rightarrow> ('r3, 'b \<times> 'r2) argument_types \<Rightarrow> ('a \<longmapsto> 'b) \<Rightarrow> ('r1 \<longmapsto> 'r3)"
   where "op_call args rets f = (\<lambda>(h,r1). case assemble_arg args r1 of (a,r2) \<Rightarrow>
@@ -1163,16 +1201,16 @@ definition op_call :: " ('r1, 'a \<times> 'r2) argument_types \<Rightarrow> ('r3
         | PartialCorrect \<Rightarrow> PartialCorrect | Fail \<Rightarrow> Fail))"
 
 lemma op_call:
-  "Arguments \<tort_lbrace>sh \<tycolon> SH\<tort_rbrace> \<tort_lbrace>a \<tycolon> A\<tort_rbrace> R args \<Longrightarrow>
-   Arguments \<tort_lbrace>sh' \<tycolon> SH'\<tort_rbrace> \<tort_lbrace>b \<tycolon> B\<tort_rbrace> R rets \<Longrightarrow>
-   \<^bold>f\<^bold>u\<^bold>n\<^bold>c f \<blangle> a \<tycolon> A \<longmapsto> b \<tycolon> B \<brangle> \<Longrightarrow>
-   \<^bold>p\<^bold>r\<^bold>o\<^bold>c op_call args rets f \<blangle> sh \<tycolon> SH \<longmapsto> sh' \<tycolon> SH' \<brangle>"
+  "Arguments SH A R args \<Longrightarrow>
+   Arguments SH' B R rets \<Longrightarrow>
+   \<^bold>f\<^bold>u\<^bold>n\<^bold>c f \<blangle> A \<longmapsto> B \<brangle> \<Longrightarrow>
+   \<^bold>p\<^bold>r\<^bold>o\<^bold>c op_call args rets f \<blangle> SH \<longmapsto> SH' \<brangle>"
   unfolding Procedure_def Function_def op_call_def Arguments_def
   by (cases args, cases rets) (auto 0 5 simp add: pair_forall split: state.split prod.split)
 
 lemma rename_func: "f \<equiv> f' \<Longrightarrow> \<^bold>f\<^bold>u\<^bold>n\<^bold>c f' \<blangle> U \<longmapsto> \<R> \<brangle> \<Longrightarrow> \<^bold>f\<^bold>u\<^bold>n\<^bold>c f \<blangle> U \<longmapsto> \<R> \<brangle>" by blast
 
-subsubsection \<open>Recursive Function\<close>
+(* subsubsection \<open>Recursive Function\<close>
 
 lemma NuAddition_auto_func_no_prems: "\<^bold>f\<^bold>u\<^bold>n\<^bold>c f \<blangle> x \<tycolon> T \<and>\<^sup>\<nu>\<^sub>a\<^sub>u\<^sub>t\<^sub>o P \<longmapsto> Y \<brangle> \<equiv> (P \<longrightarrow> \<^bold>f\<^bold>u\<^bold>n\<^bold>c f \<blangle> x \<tycolon> T \<longmapsto> Y \<brangle>)"
   unfolding Auto_def Procedure_def Function_def atomize_eq by (simp add: nu_exps) blast
@@ -1181,7 +1219,7 @@ lemma NuAddition_anti_auto: "(P \<Longrightarrow> \<^bold>f\<^bold>u\<^bold>n\<^
   by (simp add: Premise_def atomize_imp)
 lemma recursive_func_help_1: "\<^bold>f\<^bold>u\<^bold>n\<^bold>c f \<blangle> x \<tycolon> A \<and>\<^sup>\<nu>\<^sub>a\<^sub>u\<^sub>t\<^sub>o P \<longmapsto> B\<brangle> \<Longrightarrow> P \<longrightarrow> \<^bold>f\<^bold>u\<^bold>n\<^bold>c f \<blangle> x \<tycolon> A \<longmapsto> B \<brangle>"
   by (simp add: Premise_def)
-
+*)
 subsection \<open>Auto construct & destruct\<close>
 
 definition AutoConstruct :: " 'exp \<Rightarrow> ('a::lrep \<longmapsto> 'b::lrep) \<Rightarrow> (heap \<times> 'a) set \<Rightarrow> (heap \<times> 'b) set \<Rightarrow> bool "("\<^bold>c\<^bold>o\<^bold>n\<^bold>s\<^bold>t\<^bold>r\<^bold>u\<^bold>c\<^bold>t _/ \<^bold>b\<^bold>y \<^bold>p\<^bold>r\<^bold>o\<^bold>c _/ (2\<blangle>_/ \<longmapsto> _ \<brangle>)" [20,101,10,10] 100)
@@ -1318,6 +1356,7 @@ lemma op_init_register:
       \<Longrightarrow> \<^bold>p\<^bold>r\<^bold>o\<^bold>c op_init_registers idx \<blangle> S \<longmapsto> RegisterCollection (S' \<^bold>a\<^bold>n\<^bold>d R) \<brangle>"
   unfolding RegisterCollection_def op_init_registers_def \<nu>def \<nu>index_def by auto
 *)
+
 subsection \<open>Structural Pairs\<close>
 
 definition StructuralTag ("<Structural> _" [10] 9) where "StructuralTag \<equiv> Trueprop"
@@ -1372,13 +1411,40 @@ translations "_linebreak_collection_ P Q" <= "CONST AndFact P Q"
 translations "P" <= "CONST AndFact P (CONST NoFact)"
 
 *)
+
+subsection \<open>Convergence\<close>
+
+definition SameNuTy :: " 'a set \<Rightarrow> 'a set \<Rightarrow> bool " where "SameNuTy A B = True"
+text \<open>Technical tag for reasoner converges \<nu>-types of two typings.\<close>
+
+lemma [\<nu>intro 2000]: "SameNuTy \<tort_lbrace>x \<tycolon> T\<tort_rbrace> \<tort_lbrace>x' \<tycolon> T\<tort_rbrace>"
+  unfolding SameNuTy_def ..
+
+lemma [\<nu>intro 2000]: "SameNuTy A A' \<Longrightarrow> SameNuTy B B' \<Longrightarrow> SameNuTy (A\<heavy_comma> B) (A'\<heavy_comma> B')"
+  unfolding SameNuTy_def ..
+
+lemma [\<nu>intro 2000]: "SameNuTy A A' \<Longrightarrow> SameNuTy B B' \<Longrightarrow> SameNuTy (A \<heavy_asterisk> B) (A' \<heavy_asterisk> B')"
+  unfolding SameNuTy_def ..
+
+lemma [\<nu>intro 2000]: "SameNuTy A A' \<Longrightarrow> SameNuTy B B' \<Longrightarrow> SameNuTy (A\<heavy_comma> \<^bold>h\<^bold>e\<^bold>a\<^bold>p B) (A'\<heavy_comma> \<^bold>h\<^bold>e\<^bold>a\<^bold>p B')"
+  unfolding SameNuTy_def ..
+
+lemma [\<nu>intro 2000]: "(\<And>x. SameNuTy (A x) (A' x)) \<Longrightarrow> SameNuTy (ExSet A) (ExSet A')"
+  unfolding SameNuTy_def ..
+
+lemma [\<nu>intro 2000]: "SameNuTy A A' \<Longrightarrow> SameNuTy (A \<and>\<^sup>s P) (A' \<and>\<^sup>s P)"
+  unfolding SameNuTy_def ..
+
+lemma [\<nu>intro 1000]: "SameNuTy A A" \<comment> \<open>The fallback\<close>
+  unfolding SameNuTy_def ..
+
+
 section \<open>Main implementation of the system\<close>
 
 ML_file NuBasics.ML
-ML_file "./general/binary_tree.ML"
+(* ML_file "./general/binary_tree.ML" *)
 ML_file "./general/auto_level.ML"
 (* ML_file "./library/path.ML" *)
-ML \<open>Syntax.parse_term @{context} "xxx"\<close>
 ML_file \<open>library/application.ML\<close>
 ML_file "./library/general.ML"
 ML_file "./library/instructions.ML"
@@ -1390,11 +1456,12 @@ ML_file NuSys.ML
 ML_file "./library/processors.ML"
 ML_file "./library/obtain.ML"
 ML_file "./library/QuantExpansion.ML"
-ML_file NuToplevel.ML
+ML_file_debug NuToplevel.ML
 
 section \<open>Attributes and Commands\<close>
 
 ML \<open>Theory.setup (Global_Theory.add_thms_dynamic (@{binding "\<nu>instr"}, NuInstructions.list_definitions #> map snd))  \<close>
+
 attribute_setup \<nu>instr = \<open>Scan.succeed (Thm.declaration_attribute NuInstructions.add) \<close>
   \<open>Instructions of \<nu>-system\<close>
 
@@ -1514,8 +1581,9 @@ subsection \<open>Quantification Expansion\<close>
 simproc_setup named_forall_expansion ("All (P :: 'a named 'names \<Rightarrow> bool)") =
   \<open>K (QuantExpansion.simproc_of QuantExpansion.forall_expansion)\<close>
 
-simproc_setup named_exNu_expansion ("\<tort_lbrace>x \<tycolon> ExNu (P :: 'a named 'names \<Rightarrow> ('b,'c)\<nu>)\<tort_rbrace>") =
-  \<open>K (QuantExpansion.simproc_of QuantExpansion.ExNu_expansion)\<close>
+simproc_setup named_exSet_expansion ("ExSet (P :: 'a named 'names \<Rightarrow> 'b set)") =
+  \<open>K (fn ctx => fn cterms =>
+  @{print} (QuantExpansion.simproc_of QuantExpansion.ExNu_expansion ctx (@{print} cterms)))\<close>
 
 simproc_setup named_pureAll_expansion ("Pure.all (P :: 'a named 'names \<Rightarrow> prop)") =
   \<open>K (QuantExpansion.simproc_of QuantExpansion.pure_All_expansion)\<close>
@@ -1545,17 +1613,7 @@ subsection \<open>Constructive\<close>
 
 \<nu>processor accept_proc 300 \<open>\<^bold>p\<^bold>e\<^bold>n\<^bold>d\<^bold>i\<^bold>n\<^bold>g f \<^bold>o\<^bold>n blk \<^bold>r\<^bold>e\<^bold>s\<^bold>u\<^bold>l\<^bold>t\<^bold>s \<^bold>i\<^bold>n T\<close> \<open>fn ctx => fn meta =>
   Scan.succeed (fn _ => NuSys.accept_proc meta ctx)\<close>
-(*
-\<nu>processor move_fact 50 \<open>(\<^bold>c\<^bold>u\<^bold>r\<^bold>r\<^bold>e\<^bold>n\<^bold>t blk \<^bold>r\<^bold>e\<^bold>s\<^bold>u\<^bold>l\<^bold>t\<^bold>s \<^bold>i\<^bold>n (x \<tycolon> T) \<and>\<^sup>\<nu>\<^sub>a\<^sub>u\<^sub>t\<^sub>o P)\<close>
-\<open>fn ctx => fn sequent => Scan.succeed (fn _ =>
-  let
-    val facts = Proof_Context.get_thms ctx "\<glowing_star>"
-    val ctx = Proof_Context.put_thms true ("\<glowing_star>",
-        SOME ((sequent RS @{thm extract_addition_fact_minor}) :: facts) ) ctx
-  in
-    (sequent RS @{thm extract_addition_fact_major}, ctx)
-  end)\<close>
-*)
+
 \<nu>processor "apply" 9000 \<open>P\<close> \<open> fn ctx => fn meta => NuApplicant.parser >> (fn binding => fn _ =>
   (NuSys.apply ctx (NuApplicant.applicant_thms ctx binding) meta, ctx))\<close>
 
@@ -1566,8 +1624,7 @@ subsection \<open>Constructive\<close>
   \<open>fn ctx => fn sequent => (NuApplicant.parser -- Parse.opt_attribs) >> (fn (name,attrs) => fn _ =>
     let open NuBasics
     val attrs = map (Attrib.attribute_cmd ctx o Attrib.check_src ctx) attrs
-    val ths = case try (Proof_Context.get_fact ctx) (Facts.Named (name, NONE)) of SOME x => x
-         | NONE => Proof_Context.get_fact ctx (Facts.Named (name |> apfst (fn s => s ^ "_\<nu>proc"), NONE))
+    val ths = NuApplicant.applicant_thms ctx name
     val (ths,ctx) = fold_map (Thm.proof_attributes attrs) ths ctx
     val sequent = perhaps (try (fn th => @{thm Argument_I} RS th)) sequent
     in case Seq.pull (Thm.biresolution NONE false (map (pair false) ths |> @{print}) 1 sequent)
@@ -1597,7 +1654,7 @@ subsubsection \<open>Sub-procedure\<close>
 
 subsubsection \<open>Existential elimination\<close>
 
-\<nu>processor auto_existential_elimination 50 \<open>\<^bold>c\<^bold>u\<^bold>r\<^bold>r\<^bold>e\<^bold>n\<^bold>t blk \<^bold>r\<^bold>e\<^bold>s\<^bold>u\<^bold>l\<^bold>t\<^bold>s \<^bold>i\<^bold>n \<tort_lbrace>x \<tycolon> ExNu T\<tort_rbrace>\<close>
+\<nu>processor auto_existential_elimination 50 \<open>\<^bold>c\<^bold>u\<^bold>r\<^bold>r\<^bold>e\<^bold>n\<^bold>t blk \<^bold>r\<^bold>e\<^bold>s\<^bold>u\<^bold>l\<^bold>t\<^bold>s \<^bold>i\<^bold>n ExSet T\<close>
   \<open>fn ctx => fn meta => Scan.succeed (fn () =>
     raise Process_State_Call' ((meta,ctx), NuObtain.auto_choose))\<close>
 
@@ -1606,14 +1663,15 @@ subsection \<open>Simplifiers & Resonings\<close>
 \<nu>processor \<nu>simplifier 40 \<open>\<^bold>c\<^bold>u\<^bold>r\<^bold>r\<^bold>e\<^bold>n\<^bold>t blk \<^bold>r\<^bold>e\<^bold>s\<^bold>u\<^bold>l\<^bold>t\<^bold>s \<^bold>i\<^bold>n T\<close>  \<open>NuProcessors.simplifier []\<close>
 (* \<nu>processor \<nu>simplifier_final 9999 \<open>PROP P\<close>  \<open>NuProcessors.simplifier []\<close> *)
 
-\<nu>processor move_fact 50 \<open>(\<^bold>c\<^bold>u\<^bold>r\<^bold>r\<^bold>e\<^bold>n\<^bold>t blk \<^bold>r\<^bold>e\<^bold>s\<^bold>u\<^bold>l\<^bold>t\<^bold>s \<^bold>i\<^bold>n (x \<tycolon> T) \<and>\<^sup>\<nu>\<^sub>a\<^sub>u\<^sub>t\<^sub>o P)\<close>
+\<nu>processor move_fact 50 \<open>(\<^bold>c\<^bold>u\<^bold>r\<^bold>r\<^bold>e\<^bold>n\<^bold>t blk \<^bold>r\<^bold>e\<^bold>s\<^bold>u\<^bold>l\<^bold>t\<^bold>s \<^bold>i\<^bold>n T) \<and> P\<close>
 \<open>fn ctx => fn sequent => Scan.succeed (fn _ =>
   let
+    val de_premise = perhaps (try (fn th => th RS @{thm Premise_E}))
     val facts = Proof_Context.get_thms ctx "\<glowing_star>"
     val ctx = Proof_Context.put_thms true ("\<glowing_star>",
-        SOME ((sequent RS @{thm extract_addition_fact_minor}) :: facts) ) ctx
+        SOME (de_premise (sequent RS @{thm conjunct2}) :: facts) ) ctx
   in
-    (sequent RS @{thm extract_addition_fact_major}, ctx)
+    (sequent RS @{thm conjunct1}, ctx)
   end)\<close>
 
 \<nu>processor \<nu>reason 1000 \<open>PROP P \<Longrightarrow> PROP Q\<close> \<open>fn ctx => fn sequent => Scan.succeed (fn _ =>
@@ -1630,24 +1688,21 @@ subsection \<open>Literal operations\<close>
   let val term = Syntax.read_term ctx term |> Thm.cterm_of ctx |> Simplifier.rewrite ctx |> Thm.rhs_of
   in (NuSys.auto_construct ctx term meta, ctx) end)\<close>
 
-section \<open>Mechanism III\<close>
+section \<open>Mechanism III - Additional Parts\<close>
 
 subsection \<open>Variant Cast\<close>
 
-definition Variant_Cast :: " ('stack_low, 'stack) typing \<Rightarrow> ('heap_low, 'heap) typing
-    \<Rightarrow> 'vars \<Rightarrow> ('stack_low, 'vars) \<nu> \<Rightarrow> ('heap_low, 'vars) \<nu> \<Rightarrow> bool "
-      ("\<^bold>v\<^bold>a\<^bold>r\<^bold>i\<^bold>a\<^bold>n\<^bold>t \<^bold>c\<^bold>a\<^bold>s\<^bold>t _/ \<^bold>h\<^bold>e\<^bold>a\<^bold>p _/ \<longmapsto> _/ \<tycolon> _/ \<^bold>a\<^bold>n\<^bold>d _" )
-  where "Variant_Cast stack heap insts stackTy' heapTy' \<longleftrightarrow>
-    \<tort_lbrace>stack\<tort_rbrace> = \<tort_lbrace>insts \<tycolon> stackTy'\<tort_rbrace> \<and> \<tort_lbrace>heap\<tort_rbrace> = \<tort_lbrace>insts \<tycolon> heapTy'\<tort_rbrace>"
+definition Variant_Cast :: " 'vars \<Rightarrow> 'low set \<Rightarrow> ('vars \<Rightarrow> 'low set) \<Rightarrow> bool "
+      ("\<^bold>v\<^bold>a\<^bold>r\<^bold>i\<^bold>a\<^bold>n\<^bold>t _ \<^bold>i\<^bold>n _/ \<longmapsto> _" )
+  where "Variant_Cast insts S S' \<longleftrightarrow> S = S' insts"
 
 lemma Variant_Cast_I:
-  "s = pattern\<^sub>s vars \<Longrightarrow> h = pattern\<^sub>h vars \<Longrightarrow>
-  Variant_Cast (s \<tycolon> S) (h \<tycolon> H) vars (S <auto-down-lift> pattern\<^sub>s) (H <auto-down-lift> pattern\<^sub>h)"
+  "S = S' vars \<Longrightarrow> Variant_Cast vars S S' "
   unfolding Variant_Cast_def by auto
 
 lemma Variant_Cast_I_always:
-  "s = pattern\<^sub>s vars \<Longrightarrow> h = pattern\<^sub>h vars \<Longrightarrow> \<^bold>p\<^bold>r\<^bold>e\<^bold>m\<^bold>i\<^bold>s\<^bold>e always vars \<Longrightarrow>
-  Variant_Cast (s \<tycolon> S) (h \<tycolon> H) vars (S <auto-down-lift> pattern\<^sub>s <auto-where> Collect always) (H <auto-down-lift> pattern\<^sub>h)"
+  "S = S' vars \<Longrightarrow> \<^bold>p\<^bold>r\<^bold>e\<^bold>m\<^bold>i\<^bold>s\<^bold>e always vars \<Longrightarrow>
+  Variant_Cast vars S (\<lambda>vars. S' vars \<and>\<^sup>s always vars)"
   unfolding Variant_Cast_def Auto_def by (auto simp add: nu_exps)
 
 definition Variants_Quant_Tag :: " ('vars \<Rightarrow> unit) \<Rightarrow> 'a \<Rightarrow> 'a" ("<expand'_vars>")
@@ -1663,7 +1718,7 @@ lemma case_named_expn_I: "A = B x \<Longrightarrow> A = case_named B (tag x)" by
 
 ML_file_debug \<open>library/variables_tag.ML\<close>
 
-\<nu>processor vars_by_pattern 110 \<open>Variant_Cast (s \<tycolon> S) (h \<tycolon> H) vars S' H' \<Longrightarrow> PROP P\<close> \<open>fn ctx => fn meta => 
+\<nu>processor vars_by_pattern 110 \<open>Variant_Cast vars S S' \<Longrightarrow> PROP P\<close> \<open>fn ctx => fn meta => 
 let open Parse Scan NuHelp NuBasics in
   ($$$ "var" |-- list1 params -- option ($$$ "in" |-- list1 term) -- option ($$$ "heap" |-- list1 term) -- Scan.option ($$$ "always" |-- term))
     >> (fn ((((vars, stack_schema), heap_schema)), always) => fn _ =>
