NuBasicAbstractors.thy
@@ -63,24 +63,44 @@ lemma [elim,\<nu>elim]: "a \<R_arr_tail> xs \<ratio> Array' N \<Longrightarrow> 
   unfolding Inhabited_def[of "\<tort_lbrace>a \<R_arr_tail> xs \<tycolon> Array' N\<tort_rbrace>"]
   by (cases a) (auto simp add: lrep_exps pred_option_def list_all2_conv_all_nth)
 
-lemma Array'_to_Ref_\<nu>proc[\<nu>intro 10]:
+lemma Array'_to_Ref_\<nu>proc:
  "\<^bold>p\<^bold>r\<^bold>e\<^bold>m\<^bold>i\<^bold>s\<^bold>e i < length xs \<Longrightarrow> \<^bold>p\<^bold>r\<^bold>e\<^bold>m\<^bold>i\<^bold>s\<^bold>e (xs ! i) \<noteq> None \<Longrightarrow>
-  \<^bold>d\<^bold>e\<^bold>s\<^bold>t \<^bold>c\<^bold>a\<^bold>s\<^bold>t a \<R_arr_tail> xs \<tycolon> Array' N \<longmapsto> a \<R_arr_tail> xs[i := None] \<tycolon> Array' N \<heavy_asterisk> (a ||+ i) \<R_arr_tail> the (xs ! i) \<tycolon> Ref N"
-  unfolding Dest_def Cast_def Heap_Delimiter_def
-  apply (cases a) apply (auto simp add: nu_exps) apply (rule heap_split_by_addr_set[of _  _ "-{a ||+ i}"])
-  by (auto simp add: pred_option_def Ball_def nth_list_update)
+  \<^bold>c\<^bold>a\<^bold>s\<^bold>t a \<R_arr_tail> xs \<tycolon> Array' N \<longmapsto> a \<R_arr_tail> xs[i := None] \<tycolon> Array' N \<heavy_asterisk> (a ||+ i) \<R_arr_tail> the (xs ! i) \<tycolon> Ref N"
+  unfolding Dest_def Cast_def Heap_Divider_def
+    apply (cases a) apply (auto simp add: nu_exps) apply (rule heap_split_by_addr_set[of _  _ "-{a ||+ i}"])
+    by (auto simp add: pred_option_def Ball_def nth_list_update)
 
-lemma [\<nu>intro 30]:
+lemma [\<nu>intro]:
+ "\<^bold>p\<^bold>r\<^bold>e\<^bold>m\<^bold>i\<^bold>s\<^bold>e i < length xs \<Longrightarrow> \<^bold>p\<^bold>r\<^bold>e\<^bold>m\<^bold>i\<^bold>s\<^bold>e (xs ! i) \<noteq> None \<Longrightarrow>
+  \<medium_left_bracket>\<medium_left_bracket> \<^bold>c\<^bold>a\<^bold>s\<^bold>t a \<R_arr_tail> xs \<tycolon> Array' N \<longmapsto> a \<R_arr_tail> xs[i := None] \<tycolon> Array' N \<heavy_asterisk> \<medium_left_bracket>\<medium_left_bracket> (a ||+ i) \<R_arr_tail> the (xs ! i) \<tycolon> Ref N \<medium_right_bracket>\<medium_right_bracket> \<medium_right_bracket>\<medium_right_bracket>"
+  unfolding Cast_def Heap_Cast_Goal_def
+  using Array'_to_Ref_\<nu>proc[unfolded Cast_def] by blast
+
+lemma Ref_to_Array':
   "\<^bold>p\<^bold>r\<^bold>e\<^bold>m\<^bold>i\<^bold>s\<^bold>e i < length xs \<Longrightarrow>
-  \<^bold>i\<^bold>n\<^bold>t\<^bold>r\<^bold>o \<^bold>c\<^bold>a\<^bold>s\<^bold>t a \<R_arr_tail> xs[i := None] \<tycolon> Array' N \<heavy_asterisk> (a ||+ i) \<R_arr_tail> y \<tycolon> Ref N \<longmapsto> a \<R_arr_tail> xs[i := Some y] \<tycolon> Array' N"
-  unfolding Intro_def Cast_def Heap_Delimiter_def
+  \<^bold>c\<^bold>a\<^bold>s\<^bold>t a \<R_arr_tail> xs[i := None] \<tycolon> Array' N \<heavy_asterisk> (a ||+ i) \<R_arr_tail> y \<tycolon> Ref N \<longmapsto> a \<R_arr_tail> xs[i := Some y] \<tycolon> Array' N"
+  unfolding Intro_def Cast_def Heap_Divider_def Heap_Cast_Goal_def
   apply (cases a) apply (auto simp add: pred_option_def Ball_def nu_exps)
   by (metis MemAddrState_add_I1 MemAddrState_add_I2 nth_list_update option.sel)
+
+lemma [\<nu>intro]:
+ "\<^bold>p\<^bold>r\<^bold>e\<^bold>m\<^bold>i\<^bold>s\<^bold>e i < length xs \<Longrightarrow> \<^bold>p\<^bold>r\<^bold>e\<^bold>m\<^bold>i\<^bold>s\<^bold>e (xs ! i) \<noteq> None \<Longrightarrow>
+  \<medium_left_bracket>\<medium_left_bracket> \<^bold>c\<^bold>a\<^bold>s\<^bold>t a \<R_arr_tail> xs \<tycolon> Array' N \<longmapsto> a \<R_arr_tail> xs[i := None] \<tycolon> Array' N \<heavy_asterisk> \<medium_left_bracket>\<medium_left_bracket> (a ||+ i) \<R_arr_tail> the (xs ! i) \<tycolon> Ref N \<medium_right_bracket>\<medium_right_bracket> \<^bold>w\<^bold>i\<^bold>t\<^bold>h True
+      \<^bold>d\<^bold>u\<^bold>a\<^bold>l a \<R_arr_tail> xs[i := None] \<tycolon> Array' N \<heavy_asterisk> \<medium_left_bracket>\<medium_left_bracket> (a ||+ i) \<R_arr_tail> y \<tycolon> Ref N \<medium_right_bracket>\<medium_right_bracket> \<longmapsto> a \<R_arr_tail> xs[i := Some y] \<tycolon> Array' N \<medium_right_bracket>\<medium_right_bracket>"
+  unfolding Heap_Cast_Goal_def
+  by (blast intro: CastDual_I Ref_to_Array' Array'_to_Ref_\<nu>proc)
+
+(* lemma Ref_to_Array':
+  "\<medium_left_bracket>\<medium_left_bracket> \<^bold>c\<^bold>a\<^bold>s\<^bold>t H1 \<longmapsto> H2 \<heavy_asterisk> \<medium_left_bracket>\<medium_left_bracket> (a ||+ i) \<R_arr_tail> y \<tycolon> Ref N \<medium_right_bracket>\<medium_right_bracket> \<^bold>w\<^bold>i\<^bold>t\<^bold>h P1 \<medium_right_bracket>\<medium_right_bracket> \<Longrightarrow>
+  \<medium_left_bracket>\<medium_left_bracket> \<^bold>c\<^bold>a\<^bold>s\<^bold>t H2 \<longmapsto> H3 \<heavy_asterisk> \<medium_left_bracket>\<medium_left_bracket> a \<R_arr_tail> xs[i := None] \<tycolon> Array' N \<medium_right_bracket>\<medium_right_bracket> \<^bold>w\<^bold>i\<^bold>t\<^bold>h P2 \<medium_right_bracket>\<medium_right_bracket> \<Longrightarrow>
+  \<^bold>p\<^bold>r\<^bold>e\<^bold>m\<^bold>i\<^bold>s\<^bold>e i < length xs \<Longrightarrow>
+  \<medium_left_bracket>\<medium_left_bracket> \<^bold>c\<^bold>a\<^bold>s\<^bold>t H1  \<longmapsto> H3 \<heavy_asterisk> \<medium_left_bracket>\<medium_left_bracket> a \<R_arr_tail> xs[i := Some y] \<tycolon> Array' N \<medium_right_bracket>\<medium_right_bracket> \<^bold>w\<^bold>i\<^bold>t\<^bold>h P1 \<and> P2 \<medium_right_bracket>\<medium_right_bracket>" *)
+
 
 lemma split_cast_Array'_\<nu>app[\<nu>overload split_cast]:
   "\<^bold>p\<^bold>a\<^bold>r\<^bold>a\<^bold>m n \<Longrightarrow> \<^bold>p\<^bold>r\<^bold>e\<^bold>m\<^bold>i\<^bold>s\<^bold>e n < length l \<Longrightarrow>
   \<^bold>c\<^bold>a\<^bold>s\<^bold>t a \<R_arr_tail> l \<tycolon> Array' T \<longmapsto> a \<R_arr_tail> take n l \<tycolon> Array' T \<heavy_asterisk> (a ||+ n) \<R_arr_tail> drop n l \<tycolon> Array' T"
-  unfolding Cast_def Premise_def Heap_Delimiter_def apply (cases a) apply (auto simp add: nu_exps min_absorb2) 
+  unfolding Cast_def Premise_def Heap_Divider_def apply (cases a) apply (auto simp add: nu_exps min_absorb2) 
   subgoal for base ofs v
     apply (rule heap_split_by_set[of _ _ "{ MemAddress (base |+ ofs + i) | i. i < n}"])
     apply (auto simp add: pred_option_def Ball_def split: option.split)
@@ -132,10 +152,28 @@ lemma [simp]: "i < length l \<Longrightarrow> (mapSome l) [i := Some v] = mapSom
 lemma [simp]: "i < length l \<Longrightarrow> the (mapSome l ! i) = l ! i" unfolding mapSome_def by auto
 
 
-lemma [\<nu>intro 50]: "\<^bold>p\<^bold>r\<^bold>e\<^bold>m\<^bold>i\<^bold>s\<^bold>e xs' = mapSome xs2 \<Longrightarrow> \<^bold>i\<^bold>n\<^bold>t\<^bold>r\<^bold>o \<^bold>c\<^bold>a\<^bold>s\<^bold>t  a \<R_arr_tail> xs' \<tycolon> Array' N \<longmapsto> a \<R_arr_tail> xs2 \<tycolon> Array N"
+lemma Array'_cast_Array: "\<^bold>p\<^bold>r\<^bold>e\<^bold>m\<^bold>i\<^bold>s\<^bold>e xs' = mapSome xs2 \<Longrightarrow> \<^bold>c\<^bold>a\<^bold>s\<^bold>t a \<R_arr_tail> xs' \<tycolon> Array' N \<longmapsto> a \<R_arr_tail> xs2 \<tycolon> Array N"
   unfolding Cast_def Intro_def Array_def by (cases a) (auto simp add: pred_option_def Ball_def)
-lemma [\<nu>intro 10]: "\<^bold>d\<^bold>e\<^bold>s\<^bold>t \<^bold>c\<^bold>a\<^bold>s\<^bold>t a \<R_arr_tail> xs \<tycolon> Array N \<longmapsto> a \<R_arr_tail> mapSome xs \<tycolon> Array' N"
+lemma Array_cast_Array': "\<^bold>c\<^bold>a\<^bold>s\<^bold>t a \<R_arr_tail> xs \<tycolon> Array N \<longmapsto> a \<R_arr_tail> mapSome xs \<tycolon> Array' N"
   unfolding Cast_def Dest_def Array_def by (cases a) (auto simp add: pred_option_def Ball_def)
+
+lemma [\<nu>intro]:
+  "\<^bold>c\<^bold>a\<^bold>s\<^bold>t T \<longmapsto> a \<R_arr_tail> xs' \<tycolon> Array' N \<^bold>w\<^bold>i\<^bold>t\<^bold>h P \<Longrightarrow>
+   \<^bold>p\<^bold>r\<^bold>e\<^bold>m\<^bold>i\<^bold>s\<^bold>e xs' = mapSome xs2 \<Longrightarrow>
+   \<^bold>c\<^bold>a\<^bold>s\<^bold>t T \<longmapsto> a \<R_arr_tail> xs2 \<tycolon> Array N \<^bold>w\<^bold>i\<^bold>t\<^bold>h P"
+  unfolding Cast_def using Array'_cast_Array[unfolded Cast_def] by blast
+
+lemma [\<nu>intro]:
+  "\<^bold>c\<^bold>a\<^bold>s\<^bold>t a \<R_arr_tail> mapSome xs \<tycolon> Array' N \<longmapsto> T \<^bold>w\<^bold>i\<^bold>t\<^bold>h P \<Longrightarrow>
+   \<^bold>c\<^bold>a\<^bold>s\<^bold>t a \<R_arr_tail> xs \<tycolon> Array N \<longmapsto> T \<^bold>w\<^bold>i\<^bold>t\<^bold>h P"
+  unfolding Cast_def using Array_cast_Array'[unfolded Cast_def] by blast
+
+lemma [\<nu>intro]:
+  "\<medium_left_bracket>\<medium_left_bracket> \<^bold>c\<^bold>a\<^bold>s\<^bold>t a \<R_arr_tail> mapSome xs \<tycolon> Array' N \<longmapsto> H \<heavy_asterisk> \<medium_left_bracket>\<medium_left_bracket> X \<medium_right_bracket>\<medium_right_bracket> \<^bold>w\<^bold>i\<^bold>t\<^bold>h P \<^bold>d\<^bold>u\<^bold>a\<^bold>l H\<^sub>m \<heavy_asterisk> \<medium_left_bracket>\<medium_left_bracket> X\<^sub>m \<medium_right_bracket>\<medium_right_bracket> \<longmapsto> a \<R_arr_tail> xs'\<^sub>m \<tycolon> Array' N \<medium_right_bracket>\<medium_right_bracket> \<Longrightarrow>
+   \<^bold>p\<^bold>r\<^bold>e\<^bold>m\<^bold>i\<^bold>s\<^bold>e xs'\<^sub>m = mapSome xs\<^sub>m \<Longrightarrow>
+   \<medium_left_bracket>\<medium_left_bracket> \<^bold>c\<^bold>a\<^bold>s\<^bold>t a \<R_arr_tail> xs \<tycolon> Array N \<longmapsto> H \<heavy_asterisk> \<medium_left_bracket>\<medium_left_bracket> X \<medium_right_bracket>\<medium_right_bracket> \<^bold>w\<^bold>i\<^bold>t\<^bold>h P \<^bold>d\<^bold>u\<^bold>a\<^bold>l H\<^sub>m \<heavy_asterisk> \<medium_left_bracket>\<medium_left_bracket> X\<^sub>m \<medium_right_bracket>\<medium_right_bracket> \<longmapsto> a \<R_arr_tail> xs\<^sub>m \<tycolon> Array N \<medium_right_bracket>\<medium_right_bracket>"
+  unfolding Heap_Cast_Goal_def  CastDual_def Cast_def
+  using Array_cast_Array'[unfolded Cast_def] Array'_cast_Array[unfolded Cast_def] by blast
 
 lemma [\<nu>intro]: "\<^bold>c\<^bold>a\<^bold>s\<^bold>t a \<R_arr_tail> [x] \<tycolon> Array T \<longmapsto> a \<R_arr_tail> x \<tycolon> Ref T"
   unfolding Cast_def Array_def by (cases a) (simp add: pred_option_def Ball_def)
@@ -175,7 +213,7 @@ proof-
     by metis 
   then show ?thesis using a0 a1 by auto
 qed
-  
+
 
 lemma [\<nu>overload nat]: 
   "\<^bold>p\<^bold>r\<^bold>e\<^bold>m\<^bold>i\<^bold>s\<^bold>e 0 < x \<Longrightarrow> \<^bold>c\<^bold>a\<^bold>s\<^bold>t x \<tycolon> \<int>['bits::len] \<longmapsto> nat x \<tycolon> \<nat>['bits]"
