NuStd_Base.thy
@@ -4,10 +4,13 @@ begin
 
 \<nu>overloads split
 
+declare Separation_assoc[simp]
+
 proc split_array[\<nu>overload split]: \<open>ptr \<tycolon> Pointer\<heavy_comma> n \<tycolon> \<nat>[size_t]\<heavy_comma> \<^bold>h\<^bold>e\<^bold>a\<^bold>p ptr \<R_arr_tail> l \<tycolon> Array T\<close>
   \<longmapsto> \<open>ptr ||+ n \<tycolon> Pointer\<heavy_comma> \<^bold>h\<^bold>e\<^bold>a\<^bold>p ptr \<R_arr_tail> take n l \<tycolon> Array T \<heavy_asterisk> (ptr ||+ n) \<R_arr_tail> drop n l \<tycolon> Array T\<close>
   premises [used]: "n < length l"
-  \<bullet> + cast_heap split_cast_\<nu>app n
+  \<bullet> + cast_heap split_cast n
   finish
+
 
 end
